aspec+access: Syscall_AC arch split
Signed-off-by: Ryan Barry <ryan.barry@unsw.edu.au>

proof/access-control/Syscall_AC.thy
@@ -6,56 +6,53 @@
 
 theory Syscall_AC
 imports
-  Ipc_AC
-  Tcb_AC
-  Interrupt_AC
-  DomainSepInv
+  ArchIpc_AC
+  ArchTcb_AC
+  ArchInterrupt_AC
+  ArchDomainSepInv
 begin
 
-context begin interpretation Arch . (*FIXME: arch_split*)
-
-definition
-  authorised_invocation :: "'a PAS \<Rightarrow> Invocations_A.invocation \<Rightarrow> 'z::state_ext state \<Rightarrow> bool"
-where
- "authorised_invocation aag i \<equiv> \<lambda>s. case i of
-     Invocations_A.InvokeUntyped i' \<Rightarrow> valid_untyped_inv i' s \<and> (authorised_untyped_inv aag i') \<and> ct_active s
-   | Invocations_A.InvokeEndpoint epptr badge can_grant can_grant_reply \<Rightarrow>
-               \<exists>ep. ko_at (Endpoint ep) epptr s \<and>
-                    (can_grant \<longrightarrow>  (\<forall>r \<in> ep_q_refs_of ep. snd r = EPRecv \<longrightarrow> is_subject aag (fst r))
-                                  \<and> aag_has_auth_to aag Grant epptr \<and> aag_has_auth_to aag Call epptr) \<and>
-                    (can_grant_reply \<longrightarrow> aag_has_auth_to aag Call epptr)
-             \<and> aag_has_auth_to aag SyncSend epptr
-   | Invocations_A.InvokeNotification ep badge \<Rightarrow> aag_has_auth_to aag Notify ep
-   | Invocations_A.InvokeReply thread slot grant \<Rightarrow>
-       (grant \<longrightarrow> is_subject aag thread) \<and> is_subject aag (fst slot) \<and> aag_has_auth_to aag Reply thread
-   | Invocations_A.InvokeTCB i' \<Rightarrow> Tcb_AI.tcb_inv_wf i' s \<and> authorised_tcb_inv aag i'
-   | Invocations_A.InvokeDomain thread slot \<Rightarrow> False
-   | Invocations_A.InvokeCNode i' \<Rightarrow> authorised_cnode_inv aag i' s \<and> is_subject aag (cur_thread s)
-           \<and> cnode_inv_auth_derivations i' s
-   | Invocations_A.InvokeIRQControl i' \<Rightarrow> authorised_irq_ctl_inv aag i'
-   | Invocations_A.InvokeIRQHandler i' \<Rightarrow> authorised_irq_hdl_inv aag i'
-   | Invocations_A.InvokeArchObject i' \<Rightarrow> valid_arch_inv i' s \<and> authorised_arch_inv aag i' \<and> ct_active s"
+definition authorised_invocation ::
+  "'a PAS \<Rightarrow> invocation \<Rightarrow> 'z :: state_ext state \<Rightarrow> bool" where
+  "authorised_invocation aag i \<equiv> \<lambda>s. case i of
+     InvokeUntyped i' \<Rightarrow> valid_untyped_inv i' s \<and> (authorised_untyped_inv aag i') \<and> ct_active s
+   | InvokeEndpoint epptr badge can_grant can_grant_reply \<Rightarrow>
+       \<exists>ep. ko_at (Endpoint ep) epptr s \<and>
+            (can_grant \<longrightarrow>  (\<forall>r \<in> ep_q_refs_of ep. snd r = EPRecv \<longrightarrow> is_subject aag (fst r)) \<and>
+                            aag_has_auth_to aag Grant epptr \<and> aag_has_auth_to aag Call epptr) \<and>
+            (can_grant_reply \<longrightarrow> aag_has_auth_to aag Call epptr) \<and>
+            aag_has_auth_to aag SyncSend epptr
+   | InvokeNotification ep badge \<Rightarrow> aag_has_auth_to aag Notify ep
+   | InvokeReply thread slot grant \<Rightarrow>
+       (grant \<longrightarrow> is_subject aag thread) \<and> is_subject aag (fst slot)
+                                         \<and> aag_has_auth_to aag Reply thread
+   | InvokeTCB i' \<Rightarrow> tcb_inv_wf i' s \<and> authorised_tcb_inv aag i'
+   | InvokeDomain thread slot \<Rightarrow> False
+   | InvokeCNode i' \<Rightarrow> authorised_cnode_inv aag i' s \<and> is_subject aag (cur_thread s)
+                                                     \<and> cnode_inv_auth_derivations i' s
+   | InvokeIRQControl i' \<Rightarrow> authorised_irq_ctl_inv aag i'
+   | InvokeIRQHandler i' \<Rightarrow> authorised_irq_hdl_inv aag i'
+   | InvokeArchObject i' \<Rightarrow> valid_arch_inv i' s \<and> authorised_arch_inv aag i' \<and> ct_active s"
 
 lemma perform_invocation_pas_refined:
-  "\<lbrace>pas_refined aag and pas_cur_domain aag
-          and einvs and simple_sched_action and valid_invocation oper
-          and is_subject aag \<circ> cur_thread
-          and authorised_invocation aag oper\<rbrace>
-    perform_invocation blocking calling oper
+  "\<lbrace>pas_refined aag and pas_cur_domain aag and einvs and simple_sched_action
+                    and valid_invocation oper and is_subject aag \<circ> cur_thread
+                    and authorised_invocation aag oper\<rbrace>
+   perform_invocation blocking calling oper
    \<lbrace>\<lambda>rv. pas_refined aag\<rbrace>"
   apply (cases oper, simp_all)
-  apply (simp add: authorised_invocation_def validE_R_def[symmetric] invs_valid_objs
-       | wp invoke_untyped_pas_refined send_ipc_pas_refined send_signal_pas_refined
-            do_reply_transfer_pas_refined invoke_tcb_pas_refined invoke_cnode_pas_refined
-            invoke_irq_control_pas_refined invoke_irq_handler_pas_refined
-            invoke_arch_pas_refined decode_cnode_invocation_auth_derived
-       | fastforce)+
+           apply (simp add: authorised_invocation_def validE_R_def[symmetric] invs_valid_objs
+                  | wp invoke_untyped_pas_refined send_ipc_pas_refined send_signal_pas_refined
+                       do_reply_transfer_pas_refined invoke_tcb_pas_refined invoke_cnode_pas_refined
+                       invoke_irq_control_pas_refined invoke_irq_handler_pas_refined
+                       invoke_arch_pas_refined decode_cnode_invocation_auth_derived
+                  | fastforce)+
   done
 
 lemma ntfn_gives_obj_at:
-  "invs s \<Longrightarrow>
-   (\<exists>ntfn. ko_at (Notification ntfn) ntfnptr s
-           \<and> (\<forall>x\<in>ntfn_q_refs_of (ntfn_obj ntfn).
+  "invs s
+   \<Longrightarrow> (\<exists>ntfn. ko_at (Notification ntfn) ntfnptr s
+             \<and> (\<forall>x\<in>ntfn_q_refs_of (ntfn_obj ntfn).
                   (\<lambda>(t, rt). obj_at (\<lambda>tcb. ko_at tcb t s) t s) x)) = ntfn_at ntfnptr s"
   apply (rule iffI)
    apply (clarsimp simp: obj_at_def is_ntfn)
@@ -68,13 +65,12 @@ lemma ntfn_gives_obj_at:
 
 (* ((=) st) -- too strong, the thread state of the calling thread changes. *)
 lemma perform_invocation_respects:
-  "\<lbrace>pas_refined aag and integrity aag X st
-          and einvs and simple_sched_action and valid_invocation oper
-          and authorised_invocation aag oper
-          and is_subject aag \<circ> cur_thread
-          and (\<lambda>s. \<forall>p ko. kheap s p = Some ko \<longrightarrow> \<not> (is_tcb ko \<and> p = cur_thread st)  \<longrightarrow> kheap st p = Some ko)
-          \<rbrace>
-    perform_invocation blocking calling oper
+  "\<lbrace>pas_refined aag and integrity aag X st and einvs and simple_sched_action
+                    and valid_invocation oper and authorised_invocation aag oper
+                    and is_subject aag \<circ> cur_thread
+                    and (\<lambda>s. \<forall>p ko. kheap s p = Some ko
+                                    \<longrightarrow> \<not> (is_tcb ko \<and> p = cur_thread st)  \<longrightarrow> kheap st p = Some ko)\<rbrace>
+   perform_invocation blocking calling oper
    \<lbrace>\<lambda>rv. integrity aag X st\<rbrace>"
   supply [wp] = invoke_untyped_integrity send_ipc_integrity_autarch send_signal_respects
                 do_reply_transfer_respects invoke_tcb_respects invoke_cnode_respects
@@ -109,46 +105,37 @@ lemma perform_invocation_respects:
 
 declare AllowSend_def[simp] AllowRecv_def[simp]
 
-lemma hoare_conjunct1_R:
-  "\<lbrace> P \<rbrace> f \<lbrace> \<lambda> r s. Q r s \<and> Q' r s\<rbrace>,- \<Longrightarrow> \<lbrace> P \<rbrace> f \<lbrace> Q \<rbrace>,-"
-  apply(auto intro: hoare_post_imp_R)
-  done
-
-lemma hoare_conjunct2_R:
-  "\<lbrace> P \<rbrace> f \<lbrace> \<lambda> r s. Q r s \<and> Q' r s\<rbrace>,- \<Longrightarrow> \<lbrace> P \<rbrace> f \<lbrace> Q' \<rbrace>,-"
-  apply(auto intro: hoare_post_imp_R)
-  done
-
+(* FIXME AC: breaks for RISCV unless "real_cte_at slot" is assumed. This term appears in the RISCV
+             variant of arch_decode_inv_wf, but not in the ARM variant. We should avoid requalifying
+             it and instead have a wp rule for valid_arch_inv as part of a locale. *)
 lemma decode_invocation_authorised:
-  "\<lbrace>pas_refined aag and valid_cap cap and invs and ct_active and cte_wp_at ((=) cap) slot
-           and ex_cte_cap_to slot
-           and (\<lambda>s. \<forall>r\<in>zobj_refs cap. ex_nonz_cap_to r s)
-           and (\<lambda>s. \<forall>r\<in>cte_refs cap (interrupt_irq_node s). ex_cte_cap_to r s)
-           and (\<lambda>s. \<forall>cap \<in> set excaps. \<forall>r\<in>cte_refs (fst cap) (interrupt_irq_node s). ex_cte_cap_to r s)
-           and (\<lambda>s. \<forall>x \<in> set excaps. s \<turnstile> (fst x))
-           and (\<lambda>s. \<forall>x \<in> set excaps. \<forall>r\<in>zobj_refs (fst x). ex_nonz_cap_to r s)
-           and (\<lambda>s. \<forall>x \<in> set excaps. cte_wp_at ((=) (fst x)) (snd x) s)
-           and (\<lambda>s. \<forall>x \<in> set excaps. real_cte_at (snd x) s)
-           and (\<lambda>s. \<forall>x \<in> set excaps. ex_cte_cap_wp_to is_cnode_cap (snd x) s)
-           and (\<lambda>s. \<forall>x \<in> set excaps. cte_wp_at (interrupt_derived (fst x)) (snd x) s)
-           and (is_subject aag \<circ> cur_thread) and
-              K (is_subject aag (fst slot) \<and> pas_cap_cur_auth aag cap
-                \<and> (\<forall>slot \<in> set excaps. is_subject aag (fst (snd slot)))
-                \<and> (\<forall>slot \<in> set excaps. pas_cap_cur_auth aag (fst slot)))
-           and domain_sep_inv (pasMaySendIrqs aag) st'\<rbrace>
-    decode_invocation info_label args ptr slot cap excaps
+  "\<lbrace>pas_refined aag and valid_cap cap and invs and ct_active and (is_subject aag \<circ> cur_thread) and
+    cte_wp_at ((=) cap) slot and ex_cte_cap_to slot and domain_sep_inv (pasMaySendIrqs aag) st' and
+    (\<lambda>s. \<forall>r\<in>zobj_refs cap. ex_nonz_cap_to r s) and
+    (\<lambda>s. \<forall>r\<in>cte_refs cap (interrupt_irq_node s). ex_cte_cap_to r s) and
+    (\<lambda>s. \<forall>cap \<in> set excaps. \<forall>r\<in>cte_refs (fst cap) (interrupt_irq_node s). ex_cte_cap_to r s) and
+    (\<lambda>s. \<forall>x \<in> set excaps. s \<turnstile> (fst x)) and
+    (\<lambda>s. \<forall>x \<in> set excaps. \<forall>r\<in>zobj_refs (fst x). ex_nonz_cap_to r s) and
+    (\<lambda>s. \<forall>x \<in> set excaps. cte_wp_at ((=) (fst x)) (snd x) s) and
+    (\<lambda>s. \<forall>x \<in> set excaps. real_cte_at (snd x) s) and
+    (\<lambda>s. \<forall>x \<in> set excaps. ex_cte_cap_wp_to is_cnode_cap (snd x) s) and
+    (\<lambda>s. \<forall>x \<in> set excaps. cte_wp_at (interrupt_derived (fst x)) (snd x) s) and
+    K (is_subject aag (fst slot) \<and> pas_cap_cur_auth aag cap \<and>
+       (\<forall>slot \<in> set excaps. is_subject aag (fst (snd slot))) \<and>
+       (\<forall>slot \<in> set excaps. pas_cap_cur_auth aag (fst slot)))\<rbrace>
+   decode_invocation info_label args ptr slot cap excaps
    \<lbrace>\<lambda>rv. authorised_invocation aag rv\<rbrace>, -"
   unfolding decode_invocation_def
   apply (rule hoare_pre)
    apply (wp decode_untyped_invocation_authorised
-              decode_cnode_invocation_auth_derived
-              decode_cnode_inv_authorised
-              decode_tcb_invocation_authorised decode_tcb_inv_wf
-              decode_arch_invocation_authorised
-              | strengthen cnode_eq_strg
-              | wpc | simp add: comp_def authorised_invocation_def decode_invocation_def
-                        split del: if_split del: hoare_True_E_R
-              | wp (once) hoare_FalseE_R)+
+             decode_cnode_invocation_auth_derived
+             decode_cnode_inv_authorised
+             decode_tcb_invocation_authorised decode_tcb_inv_wf
+             decode_arch_invocation_authorised
+          | strengthen cnode_eq_strg
+          | wpc | simp add: comp_def authorised_invocation_def decode_invocation_def
+                       split del: if_split del: hoare_True_E_R
+          | wp (once) hoare_FalseE_R)+
 
   apply (clarsimp simp: aag_has_Control_iff_owns split_def aag_cap_auth_def)
   apply (cases cap, simp_all)
@@ -165,10 +152,10 @@ lemma decode_invocation_authorised:
       apply ((clarsimp simp: valid_cap_def is_cap_simps pas_refined_all_auth_is_owns
                             ex_cte_cap_wp_to_weakenE[OF _ TrueI]
                             cap_auth_conferred_def cap_rights_to_auth_def
-               | rule conjI | (subst split_paired_Ex[symmetric], erule exI)
-               | erule cte_wp_at_weakenE
-               | drule(1) bspec
-               | erule eq_no_cap_to_obj_with_diff_ref)+)[1]
+              | rule conjI | (subst split_paired_Ex[symmetric], erule exI)
+              | erule cte_wp_at_weakenE
+              | drule(1) bspec
+              | erule eq_no_cap_to_obj_with_diff_ref)+)[1]
      apply (simp only: domain_sep_inv_def)
     apply (rule impI, erule subst, rule pas_refined_sita_mem [OF sita_controlled],
            auto simp: cte_wp_at_caps_of_state)[1]
@@ -181,39 +168,22 @@ lemma decode_invocation_authorised:
   done
 
 lemma in_extended: "(u,a) \<in> fst (do_extended_op f s) \<Longrightarrow> \<exists>e. a = (trans_state (\<lambda>_. e) s)"
-   apply (clarsimp simp add: do_extended_op_def bind_def gets_def return_def get_def
-                   mk_ef_def modify_def select_f_def put_def trans_state_update')
-   apply force
-   done
+  by (fastforce simp: do_extended_op_def bind_def gets_def return_def get_def
+                      mk_ef_def modify_def select_f_def put_def trans_state_update')
 
 lemma set_thread_state_authorised[wp]:
   "\<lbrace>authorised_invocation aag i and (\<lambda>s. thread = cur_thread s) and valid_objs\<rbrace>
-     set_thread_state thread Structures_A.thread_state.Restart
+   set_thread_state thread Restart
    \<lbrace>\<lambda>rv. authorised_invocation aag i\<rbrace>"
-  apply (cases i)
-           apply (simp_all add: authorised_invocation_def)
-          apply (wp sts_valid_untyped_inv ct_in_state_set
-                    hoare_vcg_ex_lift sts_obj_at_impossible
-                  | simp)+
+  apply (cases i; simp add: authorised_invocation_def)
+          apply (wpsimp wp: sts_valid_untyped_inv ct_in_state_set
+                            hoare_vcg_ex_lift sts_obj_at_impossible)+
      apply (rename_tac cnode_invocation)
-     apply (case_tac cnode_invocation,
-            simp_all add: cnode_inv_auth_derivations_def authorised_cnode_inv_def)[1]
+     apply (case_tac cnode_invocation;
+            simp add: cnode_inv_auth_derivations_def authorised_cnode_inv_def)[1]
            apply (wp set_thread_state_cte_wp_at | simp)+
   apply (rename_tac arch_invocation)
-  apply (case_tac arch_invocation, simp_all add: valid_arch_inv_def)[1]
-      apply (rename_tac page_table_invocation)
-      apply (case_tac page_table_invocation, simp_all add: valid_pti_def)[1]
-       apply (wp sts_typ_ats sts_obj_at_impossible ct_in_state_set
-                 hoare_vcg_ex_lift hoare_vcg_conj_lift
-               | simp add: valid_pdi_def)+
-     apply (rename_tac asid_control_invocation)
-     apply (case_tac asid_control_invocation, simp_all add: valid_aci_def)
-    apply (wp ct_in_state_set | simp)+
-  apply (rename_tac asid_pool_invocation)
-  apply (case_tac asid_pool_invocation; simp add: valid_apinv_def)
-  apply (wp sts_obj_at_impossible ct_in_state_set
-            hoare_vcg_ex_lift
-          | simp)+
+  apply (wpsimp wp: sts_valid_arch_inv ct_in_state_set)
   done
 
 lemma sts_first_restart:
@@ -226,8 +196,8 @@ lemma sts_first_restart:
 
 lemma lcs_reply_owns:
   "\<lbrace>pas_refined aag and K (is_subject aag thread)\<rbrace>
-    lookup_cap_and_slot thread ptr
-   \<lbrace>\<lambda>rv s. \<forall>ep. (\<exists>m R. fst rv = cap.ReplyCap ep m R \<and> AllowGrant \<in> R) \<longrightarrow> is_subject aag ep\<rbrace>, -"
+   lookup_cap_and_slot thread ptr
+   \<lbrace>\<lambda>rv _. \<forall>ep. (\<exists>m R. fst rv = ReplyCap ep m R \<and> AllowGrant \<in> R) \<longrightarrow> is_subject aag ep\<rbrace>, -"
   apply (rule hoare_post_imp_R)
    apply (rule hoare_pre)
     apply (rule hoare_vcg_conj_lift_R [where S = "K (pas_refined aag)"])
@@ -241,21 +211,27 @@ crunch pas_refined[wp]: reply_from_kernel "pas_refined aag"
   (simp: split_def)
 
 lemma lookup_cap_and_slot_valid_fault3:
-  "\<lbrace>valid_objs\<rbrace> lookup_cap_and_slot thread cptr
-   -,
-   \<lbrace>\<lambda>ft s. valid_fault (ExceptionTypes_A.CapFault (of_bl cptr) rp ft)\<rbrace>"
+  "\<lbrace>valid_objs\<rbrace>
+   lookup_cap_and_slot thread cptr
+   -, \<lbrace>\<lambda>ft _. valid_fault (CapFault (of_bl cptr) rp ft)\<rbrace>"
   apply (unfold validE_E_def)
   apply (rule hoare_post_impErr)
     apply (rule lookup_cap_and_slot_valid_fault)
    apply auto
   done
 
-definition guarded_pas_domain
-where
+definition guarded_pas_domain where
   "guarded_pas_domain aag \<equiv>
-     \<lambda>s. cur_thread s \<noteq> idle_thread s \<longrightarrow>
-         pasObjectAbs aag (cur_thread s) \<in> pasDomainAbs aag (cur_domain s)"
+   \<lambda>s. cur_thread s \<noteq> idle_thread s
+       \<longrightarrow> pasObjectAbs aag (cur_thread s) \<in> pasDomainAbs aag (cur_domain s)"
 
+locale gpd_wps' =
+  fixes f :: "(det_ext state, 'z) nondet_monad"
+  assumes idle_thread[wp]: "\<And>P. f \<lbrace>\<lambda>s. P (idle_thread s)\<rbrace>"
+  and cur_thread[wp]: "\<And>P. f \<lbrace>\<lambda>s. P (cur_thread s)\<rbrace>"
+
+locale gpd_wps = gpd_wps' +
+  assumes cur_domain[wp]: "\<And>P. f \<lbrace>\<lambda>s. P (cur_domain s)\<rbrace>"
 
 lemma guarded_pas_domain_lift:
   assumes a: "\<And>P. \<lbrace>\<lambda>s. P (cur_thread s)\<rbrace> f \<lbrace>\<lambda>r s. P (cur_thread s)\<rbrace>"
@@ -270,49 +246,46 @@ lemma guarded_pas_domain_lift:
   done
 
 lemma guarded_to_cur_domain:
-  "\<lbrakk>invs s; ct_in_state x s; \<not> x IdleThreadState; guarded_pas_domain aag s;
-    is_subject aag (cur_thread s)\<rbrakk>
-   \<Longrightarrow> pas_cur_domain aag s"
-  by (auto simp: invs_def valid_state_def valid_idle_def pred_tcb_at_def obj_at_def
-                 ct_in_state_def guarded_pas_domain_def)
-
+  "\<lbrakk> invs s; ct_in_state x s; \<not> x IdleThreadState;
+     guarded_pas_domain aag s; is_subject aag (cur_thread s) \<rbrakk>
+     \<Longrightarrow> pas_cur_domain aag s"
+  by (auto simp: invs_def valid_state_def valid_idle_def pred_tcb_at_def
+                 obj_at_def ct_in_state_def guarded_pas_domain_def)
 
 lemma handle_invocation_pas_refined:
-  shows "\<lbrace>pas_refined aag and guarded_pas_domain aag and domain_sep_inv (pasMaySendIrqs aag) st'
-          and einvs and ct_active and schact_is_rct
-          and is_subject aag \<circ> cur_thread\<rbrace>
-     handle_invocation calling blocking
-   \<lbrace>\<lambda>rv. pas_refined aag\<rbrace>"
+  "\<lbrace>pas_refined aag and guarded_pas_domain aag and domain_sep_inv (pasMaySendIrqs aag) st'
+                    and einvs and ct_active and schact_is_rct and is_subject aag \<circ> cur_thread\<rbrace>
+   handle_invocation calling blocking
+   \<lbrace>\<lambda>_. pas_refined aag\<rbrace>"
   apply (simp add: handle_invocation_def split_def)
   apply (cases blocking, simp)
-   apply (rule hoare_pre)
-    by (((wp syscall_valid without_preemption_wp
-              handle_fault_pas_refined set_thread_state_pas_refined
-              set_thread_state_runnable_valid_sched
-              perform_invocation_pas_refined
-              hoare_vcg_conj_lift hoare_vcg_all_lift
-         | wpc
-         | rule hoare_drop_imps
-         | simp add: if_apply_def2 conj_comms split del: if_split
+  by (((wp syscall_valid without_preemption_wp
+           handle_fault_pas_refined set_thread_state_pas_refined
+           set_thread_state_runnable_valid_sched
+           perform_invocation_pas_refined
+           hoare_vcg_conj_lift hoare_vcg_all_lift
+        | wpc
+        | rule hoare_drop_imps
+        | simp add: if_apply_def2 conj_comms split del: if_split
                del: hoare_True_E_R)+),
-        ((wp lookup_extra_caps_auth lookup_extra_caps_authorised
-              decode_invocation_authorised
-              lookup_cap_and_slot_authorised
-              lookup_cap_and_slot_cur_auth
-              as_user_pas_refined
-              lookup_cap_and_slot_valid_fault3
+       ((wp lookup_extra_caps_auth lookup_extra_caps_authorised
+            decode_invocation_authorised
+            lookup_cap_and_slot_authorised
+            lookup_cap_and_slot_cur_auth
+            as_user_pas_refined
+            lookup_cap_and_slot_valid_fault3
          | simp add: comp_def runnable_eq_active)+),
-         (auto intro: guarded_to_cur_domain
-               simp: ct_in_state_def st_tcb_at_def live_def hyp_live_def
-               intro: if_live_then_nonz_capD)[1])+
+       (auto intro: guarded_to_cur_domain
+              simp: ct_in_state_def st_tcb_at_def live_def
+             intro: if_live_then_nonz_capD)[1])+
 
 lemma handle_invocation_respects:
-  "\<lbrace>integrity aag X st and pas_refined aag and guarded_pas_domain aag and domain_sep_inv (pasMaySendIrqs aag) st'
-          and einvs and ct_active and schact_is_rct
-          and is_subject aag \<circ> cur_thread
-          and ((=) st)\<rbrace>
-     handle_invocation calling blocking
-   \<lbrace>\<lambda>rv. integrity aag X st\<rbrace>"
+  "\<lbrace>integrity aag X st and pas_refined aag and guarded_pas_domain aag
+                       and domain_sep_inv (pasMaySendIrqs aag) st'
+                       and einvs and ct_active and schact_is_rct
+                       and is_subject aag \<circ> cur_thread and ((=) st)\<rbrace>
+   handle_invocation calling blocking
+   \<lbrace>\<lambda>_. integrity aag X st\<rbrace>"
   apply (simp add: handle_invocation_def split_def)
   apply (wp syscall_valid without_preemption_wp handle_fault_integrity_autarch
             reply_from_kernel_integrity_autarch
@@ -324,85 +297,74 @@ lemma handle_invocation_respects:
          | simp add: if_apply_def2
                 split del: if_split)+
          apply (simp add: conj_comms pred_conj_def comp_def if_apply_def2 split del: if_split
-               | wp perform_invocation_respects set_thread_state_pas_refined
-                  set_thread_state_authorised
-                  set_thread_state_runnable_valid_sched
-                  set_thread_state_integrity_autarch
-                  sts_first_restart
-                  decode_invocation_authorised
-                  lookup_extra_caps_auth lookup_extra_caps_authorised
-                  set_thread_state_integrity_autarch
-                  lookup_cap_and_slot_cur_auth lookup_cap_and_slot_authorised
-                  hoare_vcg_const_imp_lift perform_invocation_pas_refined
-                  set_thread_state_ct_st      hoare_vcg_const_imp_lift_R
-                  lookup_cap_and_slot_valid_fault3
-               | (rule valid_validE, strengthen invs_vobjs_strgs))+
+                | wp perform_invocation_respects set_thread_state_pas_refined
+                   set_thread_state_authorised
+                   set_thread_state_runnable_valid_sched
+                   set_thread_state_integrity_autarch
+                   sts_first_restart
+                   decode_invocation_authorised
+                   lookup_extra_caps_auth lookup_extra_caps_authorised
+                   set_thread_state_integrity_autarch
+                   lookup_cap_and_slot_cur_auth lookup_cap_and_slot_authorised
+                   hoare_vcg_const_imp_lift perform_invocation_pas_refined
+                   set_thread_state_ct_st hoare_vcg_const_imp_lift_R
+                   lookup_cap_and_slot_valid_fault3
+                | (rule valid_validE, strengthen invs_vobjs_strgs))+
   by (fastforce intro: st_tcb_ex_cap' guarded_to_cur_domain
                  simp: ct_in_state_def runnable_eq_active)
 
 crunch pas_refined[wp]: delete_caller_cap "pas_refined aag"
 
-lemma invs_sym_refs_strg:
-  "invs s \<longrightarrow> sym_refs (state_refs_of s)" by clarsimp
-
 lemma handle_recv_pas_refined:
   "\<lbrace>pas_refined aag and invs and is_subject aag \<circ> cur_thread\<rbrace>
      handle_recv is_blocking
-   \<lbrace>\<lambda>rv. pas_refined aag\<rbrace>"
+   \<lbrace>\<lambda>_. pas_refined aag\<rbrace>"
   apply (simp add: handle_recv_def Let_def lookup_cap_def split_def)
   apply (wp handle_fault_pas_refined receive_ipc_pas_refined receive_signal_pas_refined
             get_cap_auth_wp [where aag=aag] lookup_slot_for_cnode_op_authorised
             lookup_slot_for_thread_authorised lookup_slot_for_thread_cap_fault
             hoare_vcg_all_lift_R get_simple_ko_wp
-       | wpc | simp
-       | (rule_tac Q="\<lambda>rv s. invs s \<and> is_subject aag thread
-                             \<and> (pasSubject aag, Receive, pasObjectAbs aag thread) \<in> pasPolicy aag"
-                in hoare_strengthen_post,
-          wp, clarsimp simp: invs_valid_objs invs_sym_refs))+
-     apply (rule_tac Q' = "\<lambda>rv s. pas_refined aag s \<and> invs s \<and> tcb_at thread s
-                                   \<and> cur_thread s = thread \<and> is_subject aag (cur_thread s)
-                                   \<and> is_subject aag thread" in hoare_post_imp_R [rotated])
+         | wpc | simp
+         | (rule_tac Q="\<lambda>rv s. invs s \<and> is_subject aag thread \<and> aag_has_auth_to aag Receive thread"
+                  in hoare_strengthen_post,
+            wp, clarsimp simp: invs_valid_objs invs_sym_refs))+
+     apply (rule_tac Q'="\<lambda>rv s. pas_refined aag s \<and> invs s \<and> tcb_at thread s
+                              \<and> cur_thread s = thread \<and> is_subject aag (cur_thread s)
+                              \<and> is_subject aag thread" in hoare_post_imp_R [rotated])
       apply (fastforce simp: aag_cap_auth_def cap_auth_conferred_def
                              cap_rights_to_auth_def valid_fault_def)
-     apply (wp user_getreg_inv | strengthen invs_vobjs_strgs invs_sym_refs_strg | simp)+
+     apply (wp user_getreg_inv | strengthen invs_vobjs_strgs | simp)+
   apply clarsimp
   done
 
 crunch respects[wp]: delete_caller_cap "integrity aag X st"
 
-lemma invs_mdb_strgs: "invs s \<longrightarrow> valid_mdb s"
-  by auto
-
 lemma handle_recv_integrity:
   "\<lbrace>integrity aag X st and pas_refined aag and einvs and is_subject aag \<circ> cur_thread
-      and K(valid_mdb st \<and> valid_objs st)\<rbrace>
-     handle_recv is_blocking
-   \<lbrace>\<lambda>rv. integrity aag X st\<rbrace>"
+                       and K (valid_mdb st \<and> valid_objs st)\<rbrace>
+   handle_recv is_blocking
+   \<lbrace>\<lambda>_. integrity aag X st\<rbrace>"
   apply (rule hoare_gen_asm)
   apply (simp add: handle_recv_def Let_def lookup_cap_def split_def)
   apply (wp handle_fault_integrity_autarch receive_ipc_integrity_autarch
             receive_signal_integrity_autarch lookup_slot_for_thread_authorised
             lookup_slot_for_thread_cap_fault get_cap_auth_wp [where aag=aag] get_simple_ko_wp
-        | wpc
-        | simp
-        | rule_tac Q="\<lambda>rv s. invs s \<and> is_subject aag thread
-                           \<and> (pasSubject aag, Receive, pasObjectAbs aag thread) \<in> pasPolicy aag"
-                in hoare_strengthen_post, wp, clarsimp simp: invs_valid_objs invs_sym_refs)+
-     apply (rule_tac Q' = "\<lambda>rv s. pas_refined aag s \<and> einvs s \<and> is_subject aag (cur_thread s)
-                         \<and> tcb_at thread s \<and> cur_thread s = thread
-            \<and> is_subject aag thread \<and> integrity aag X st s" in hoare_post_imp_R [rotated])
+         | wpc
+         | simp
+         | rule_tac Q="\<lambda>rv s. invs s \<and> is_subject aag thread \<and> aag_has_auth_to aag Receive thread"
+                 in hoare_strengthen_post, wp, clarsimp simp: invs_valid_objs invs_sym_refs)+
+     apply (rule_tac Q'="\<lambda>rv s. pas_refined aag s \<and> einvs s \<and> is_subject aag (cur_thread s)
+                              \<and> tcb_at thread s \<and> cur_thread s = thread \<and> is_subject aag thread
+                              \<and> integrity aag X st s" in hoare_post_imp_R [rotated])
       apply (fastforce simp: aag_cap_auth_def cap_auth_conferred_def
                              cap_rights_to_auth_def valid_fault_def)
-     apply (wp user_getreg_inv
-           | strengthen invs_vobjs_strgs invs_sym_refs_strg invs_mdb_strgs
-           | simp)+
-  apply clarsimp
+     apply wpsimp+
   done
 
 lemma handle_reply_pas_refined[wp]:
-  "\<lbrace> pas_refined aag and invs and is_subject aag \<circ> cur_thread\<rbrace>
-     handle_reply
-   \<lbrace>\<lambda>rv. pas_refined aag\<rbrace>"
+  "\<lbrace>pas_refined aag and invs and is_subject aag \<circ> cur_thread\<rbrace>
+   handle_reply
+   \<lbrace>\<lambda>_. pas_refined aag\<rbrace>"
   unfolding handle_reply_def
   apply (rule hoare_pre)
    apply (wp do_reply_transfer_pas_refined get_cap_auth_wp [where aag = aag]| wpc)+
@@ -410,11 +372,9 @@ lemma handle_reply_pas_refined[wp]:
            intro: aag_Control_into_owns)
 
 lemma handle_reply_respects:
-  "\<lbrace>integrity aag X st and pas_refined aag
-          and einvs
-          and is_subject aag \<circ> cur_thread\<rbrace>
-     handle_reply
-   \<lbrace>\<lambda>rv. integrity aag X st\<rbrace>"
+  "\<lbrace>integrity aag X st and pas_refined aag and einvs and is_subject aag \<circ> cur_thread\<rbrace>
+   handle_reply
+   \<lbrace>\<lambda>_. integrity aag X st\<rbrace>"
   unfolding handle_reply_def
   apply (rule hoare_pre)
   apply (wp do_reply_transfer_respects get_cap_auth_wp [where aag = aag]| wpc)+
@@ -425,9 +385,7 @@ lemma handle_reply_respects:
   done
 
 lemma ethread_set_time_slice_pas_refined[wp]:
-  "\<lbrace>pas_refined aag\<rbrace>
-     ethread_set (tcb_time_slice_update f) thread
-   \<lbrace>\<lambda>rv. pas_refined aag\<rbrace>"
+  "ethread_set (tcb_time_slice_update f) thread \<lbrace>pas_refined aag\<rbrace>"
   apply (simp add: ethread_set_def set_eobject_def | wp)+
   apply (clarsimp simp: pas_refined_def tcb_domain_map_wellformed_aux_def)
   apply (erule_tac x="(a, b)" in ballE)
@@ -438,16 +396,11 @@ lemma ethread_set_time_slice_pas_refined[wp]:
   done
 
 lemma thread_set_time_slice_pas_refined[wp]:
-  "\<lbrace>pas_refined aag\<rbrace>
-     thread_set_time_slice tptr time
-   \<lbrace>\<lambda>rv. pas_refined aag\<rbrace>"
-  apply (simp add: thread_set_time_slice_def | wp)+
-  done
+  "thread_set_time_slice tptr time \<lbrace>pas_refined aag\<rbrace>"
+  by (simp add: thread_set_time_slice_def | wp)+
 
 lemma dec_domain_time_pas_refined[wp]:
-  "\<lbrace>pas_refined aag\<rbrace>
-     dec_domain_time
-   \<lbrace>\<lambda>rv. pas_refined aag\<rbrace>"
+  "dec_domain_time \<lbrace>pas_refined aag\<rbrace>"
   apply (simp add: dec_domain_time_def | wp)+
   apply (clarsimp simp: pas_refined_def tcb_domain_map_wellformed_aux_def)
   done
@@ -455,57 +408,189 @@ lemma dec_domain_time_pas_refined[wp]:
 crunch pas_refined[wp]: timer_tick "pas_refined aag"
   (wp_del: timer_tick_extended.pas_refined_tcb_domain_map_wellformed)
 
+
+locale Syscall_AC_wps =
+  fixes f :: "(det_ext state, 'z) nondet_monad"
+  and aag :: "'a PAS"
+  assumes respects[wp]: "f \<lbrace>integrity aag X st\<rbrace>"
+  and pas_refined[wp]: "f \<lbrace>pas_refined aag\<rbrace>"
+
+locale Syscall_AC_1 =
+  fixes aag :: "'a PAS"
+  assumes invs_irq_state_update[simp]:
+    "invs ((s :: det_ext state)\<lparr>machine_state := irq_state_update f s'\<rparr>) =
+     invs (s\<lparr>machine_state := s'\<rparr>)"
+  and prepare_thread_delete_Syscall_AC_wps''[simp]:
+    "gpd_wps' (prepare_thread_delete p)"
+  and arch_finalise_cap_Syscall_AC_wps''[simp]:
+    "gpd_wps' (arch_finalise_cap acap final)"
+  and cap_move_Syscall_AC_wps''[simp]:
+    "gpd_wps' (cap_move new_cap src_slot dest_slot)"
+  and cancel_badged_sends_Syscall_AC_wps''[simp]:
+    "gpd_wps' (cancel_badged_sends epptr badge)"
+  and arch_post_modify_registers_Syscall_AC_wps[simp]:
+    "gpd_wps (arch_post_modify_registers cur t)"
+  and arch_perform_invocation_Syscall_AC_wps[simp]:
+    "gpd_wps (arch_perform_invocation ai)"
+  and arch_invoke_irq_control_Syscall_AC_wps[simp]:
+    "gpd_wps (arch_invoke_irq_control ivk)"
+  and arch_invoke_irq_handler_Syscall_AC_wps[simp]:
+    "gpd_wps (arch_invoke_irq_handler ihi)"
+  and arch_mask_irq_signal_Syscall_AC_wps[simp]:
+    "gpd_wps (arch_mask_irq_signal irq)"
+  and handle_reserved_irq_Syscall_AC_wps[simp]:
+    "gpd_wps (handle_reserved_irq irq)"
+  and handle_arch_fault_reply_Syscall_AC_wps[simp]:
+    "gpd_wps (handle_arch_fault_reply vmf thread x y)"
+  and handle_hypervisor_fault_Syscall_AC_wps[simp]:
+    "gpd_wps (handle_hypervisor_fault t hf_t)"
+  and handle_vm_fault_Syscall_AC_wps[simp]:
+    "gpd_wps (handle_vm_fault t vmf_t)"
+  and arch_switch_to_thread_Syscall_AC_wps'[simp]:
+    "Syscall_AC_wps (arch_switch_to_thread t) aag"
+  and arch_switch_to_idle_thread_respects[simp]:
+    "Syscall_AC_wps (arch_switch_to_idle_thread) aag"
+  and arch_activate_idle_thread_respects[simp]:
+    "Syscall_AC_wps (arch_activate_idle_thread t) aag"
+  and arch_mask_irq_signal_integrity[simp]:
+    "Syscall_AC_wps (arch_mask_irq_signal irq) aag"
+  and handle_reserved_irq_integrity[simp]:
+    "Syscall_AC_wps (handle_reserved_irq irq) aag"
+  and handle_hypervisor_fault_integrity[simp]:
+    "Syscall_AC_wps (handle_hypervisor_fault t hf_t) aag"
+  and arch_switch_to_idle_thread_pas_refined[wp]:
+    "arch_switch_to_idle_thread \<lbrace>pas_refined aag\<rbrace>"
+  and arch_activate_idle_thread_pas_refined[wp]:
+    "arch_activate_idle_thread t \<lbrace>pas_refined aag\<rbrace>"
+  and arch_mask_irq_signal_pas_refined[wp]:
+    "arch_mask_irq_signal irq \<lbrace>pas_refined aag\<rbrace>"
+  and handle_reserved_irq_pas_refined[wp]:
+    "handle_reserved_irq irq \<lbrace>pas_refined aag\<rbrace>"
+  and handle_hypervisor_fault_pas_refined[wp]:
+    "handle_hypervisor_fault t hf_t \<lbrace>pas_refined aag\<rbrace>"
+  and handle_vm_fault_integrity:
+    "\<lbrace>integrity aag X st and K (is_subject aag thread)\<rbrace>
+     handle_vm_fault thread vmfault_type
+     \<lbrace>\<lambda>rv. integrity aag X st\<rbrace>"
+  and handle_vm_fault_pas_refined[wp]:
+    "handle_vm_fault t vmf_t \<lbrace>pas_refined aag\<rbrace>"
+  and arch_mask_irq_signal_pas_cur_domain:
+    "arch_mask_irq_signal irq \<lbrace>pas_cur_domain aag\<rbrace>"
+  and handle_reserved_irq_pas_cur_domain:
+    "handle_reserved_irq irq \<lbrace>pas_cur_domain aag\<rbrace>"
+  and ackInterrupt_underlying_memory_inv[wp]:
+    "\<And>P. ackInterrupt irq \<lbrace>\<lambda>s. P (underlying_memory s)\<rbrace>"
+  and resetTimer_underlying_memory_inv[wp]:
+    "\<And>P. resetTimer \<lbrace>\<lambda>s. P (underlying_memory s)\<rbrace>"
+  and arch_post_cap_deletion_ct_active[wp]:
+    "arch_post_cap_deletion acap \<lbrace>\<lambda>s :: det_ext state. ct_active s\<rbrace>"
+  and arch_mask_irq_signal_arch_state[wp]:
+    "\<And>P. arch_mask_irq_signal irq \<lbrace>\<lambda>s :: det_ext state. P (arch_state s)\<rbrace>"
+  and handle_reserved_irq_arch_state[wp]:
+    "\<And>P. handle_reserved_irq irq \<lbrace>\<lambda>s :: det_ext state. P (arch_state s)\<rbrace>"
+  and init_arch_objects_arch_state[wp]:
+    "\<And>P. init_arch_objects new_type ptr n sz refs \<lbrace>\<lambda>s :: det_ext state. P (arch_state s)\<rbrace>"
+  and getActiveIRQ_inv:
+    "\<And>P. \<forall>f s. P s \<longrightarrow> P (irq_state_update f s)
+          \<Longrightarrow> \<lbrace>P\<rbrace> getActiveIRQ in_kernel \<lbrace>\<lambda>rv. P\<rbrace>"
+  and getActiveIRQ_rv_None:
+    "\<lbrace>\<top>\<rbrace> getActiveIRQ True \<lbrace>\<lambda>rv ms. (rv \<noteq> None \<longrightarrow> the rv \<notin> non_kernel_IRQs)\<rbrace>"
+  and set_thread_state_restart_to_running_respects:
+    "\<lbrace>integrity aag X st and st_tcb_at ((=) Restart) thread and K (pasMayActivate aag)\<rbrace>
+     do pc \<leftarrow> as_user thread getRestartPC;
+              as_user thread $ setNextPC pc;
+              set_thread_state thread Structures_A.thread_state.Running
+     od
+     \<lbrace>\<lambda>_. integrity aag X st\<rbrace>"
+begin
+
+interpretation prepare_thread_delete: gpd_wps' "prepare_thread_delete p"
+  by simp
+interpretation arch_finalise_cap: gpd_wps' "arch_finalise_cap acap final"
+  by simp
+interpretation cap_move: gpd_wps' "cap_move new_cap src_slot dest_slot"
+  by simp
+interpretation cancel_badged_sends: gpd_wps' "cancel_badged_sends epptr badge"
+  by simp
+
+interpretation arch_post_modify_registers: gpd_wps "arch_post_modify_registers cur t"
+  by simp
+interpretation arch_perform_invocation: gpd_wps "arch_perform_invocation ai"
+  by simp
+interpretation arch_invoke_irq_control: gpd_wps "arch_invoke_irq_control ivk"
+  by simp
+interpretation arch_invoke_irq_handler: gpd_wps "arch_invoke_irq_handler ihi"
+  by simp
+interpretation arch_mask_irq_signal: gpd_wps "arch_mask_irq_signal irq"
+  by simp
+interpretation handle_reserved_irq: gpd_wps "handle_reserved_irq irq"
+  by simp
+interpretation handle_arch_fault_reply: gpd_wps "handle_arch_fault_reply vmf thread x y"
+  by simp
+interpretation handle_hypervisor_fault: gpd_wps "handle_hypervisor_fault t hf_t"
+  by simp
+interpretation handle_vm_fault: gpd_wps "handle_vm_fault t vmf_t"
+  by simp
+
+interpretation arch_switch_to_thread: Syscall_AC_wps "arch_switch_to_thread t" aag
+  by simp
+interpretation arch_switch_to_idle_thread: Syscall_AC_wps "arch_switch_to_idle_thread" aag
+  by simp
+interpretation arch_activate_idle_thread: Syscall_AC_wps "arch_activate_idle_thread t" aag
+  by simp
+interpretation arch_mask_irq_signal: Syscall_AC_wps "arch_mask_irq_signal irq" aag
+  by simp
+interpretation handle_reserved_irq: Syscall_AC_wps "handle_reserved_irq irq" aag
+  by simp
+interpretation handle_hypervisor_fault: Syscall_AC_wps "handle_hypervisor_fault t hf_t" aag
+  by simp
+
 lemma handle_interrupt_pas_refined:
-  "\<lbrace>pas_refined aag\<rbrace>
-     handle_interrupt irq
-   \<lbrace>\<lambda>rv. pas_refined aag\<rbrace>"
+  "handle_interrupt irq \<lbrace>pas_refined aag\<rbrace>"
   apply (simp add: handle_interrupt_def)
   apply (rule conjI; rule impI;rule hoare_pre)
   apply (wp send_signal_pas_refined get_cap_wp
-       | wpc
-       | simp add: get_irq_slot_def get_irq_state_def handle_reserved_irq_def)+
+         | wpc
+         | simp add: get_irq_slot_def get_irq_state_def )+
   done
 
 lemma dec_domain_time_integrity[wp]:
-  "\<lbrace>integrity aag X st\<rbrace>
-        dec_domain_time
-       \<lbrace>\<lambda>_. integrity aag X st\<rbrace>"
+  "dec_domain_time \<lbrace>integrity aag X st\<rbrace>"
   apply (simp add: dec_domain_time_def | wp)+
   apply (clarsimp simp: integrity_subjects_def)
   done
 
 lemma timer_tick_integrity[wp]:
   "\<lbrace>integrity aag X st and pas_refined aag and (\<lambda>s. ct_active s \<longrightarrow> is_subject aag (cur_thread s))\<rbrace>
-        timer_tick
-       \<lbrace>\<lambda>_. integrity aag X st\<rbrace>"
+   timer_tick
+   \<lbrace>\<lambda>_. integrity aag X st\<rbrace>"
   apply (simp add: timer_tick_def)
   apply (wp ethread_set_integrity_autarch gts_wp
-           | wpc | simp add: thread_set_time_slice_def split del: if_split)+
+         | wpc | simp add: thread_set_time_slice_def split del: if_split)+
   apply (clarsimp simp: ct_in_state_def st_tcb_at_def obj_at_def)
   done
 
 lemma handle_interrupt_integrity_autarch:
-  "\<lbrace>integrity aag X st and pas_refined aag
-          and invs and (\<lambda>s. ct_active s \<longrightarrow> is_subject aag (cur_thread s))
-          and K (is_subject_irq aag irq)\<rbrace>
-     handle_interrupt irq
-   \<lbrace>\<lambda>rv. integrity aag X st\<rbrace>"
-  apply (simp add: handle_interrupt_def  cong: irq_state.case_cong maskInterrupt_def
-                   ackInterrupt_def resetTimer_def )
+  "\<lbrace>integrity aag X st and pas_refined aag and invs
+                       and (\<lambda>s. ct_active s \<longrightarrow> is_subject aag (cur_thread s))
+                       and K (is_subject_irq aag irq)\<rbrace>
+   handle_interrupt irq
+   \<lbrace>\<lambda>_. integrity aag X st\<rbrace>"
+  apply (simp add: handle_interrupt_def  cong: irq_state.case_cong)
   apply (rule conjI; rule impI; rule hoare_pre)
-  apply (wp (once) send_signal_respects get_cap_auth_wp [where aag = aag] dmo_mol_respects
-       | simp add: get_irq_slot_def get_irq_state_def ackInterrupt_def resetTimer_def
-                   handle_reserved_irq_def
-       | wp dmo_no_mem_respects
-       | wpc)+
+     apply (wp (once) send_signal_respects get_cap_auth_wp [where aag = aag] dmo_mol_respects
+                      ackInterrupt_device_state_inv resetTimer_device_state_inv
+            | simp add: get_irq_slot_def get_irq_state_def
+            | wp dmo_no_mem_respects
+            | wpc)+
   apply (fastforce simp: is_cap_simps aag_cap_auth_def cap_auth_conferred_def
                          cap_rights_to_auth_def)
   done
 
 lemma hacky_ipc_Send:
-  "\<lbrakk> (pasObjectAbs aag (interrupt_irq_node s irq), Notify, pasObjectAbs aag p) \<in> pasPolicy aag;
+  "\<lbrakk> abs_has_auth_to aag Notify (interrupt_irq_node s irq) p;
      pas_refined aag s; pasMaySendIrqs aag \<rbrakk>
-   \<Longrightarrow> aag_has_auth_to aag Notify p"
+     \<Longrightarrow> aag_has_auth_to aag Notify p"
   unfolding pas_refined_def
   apply (clarsimp simp: policy_wellformed_def irq_map_wellformed_aux_def)
   apply (drule spec [where x = "pasIRQAbs aag irq"], drule spec [where x = "pasObjectAbs aag p"],
@@ -513,20 +598,19 @@ lemma hacky_ipc_Send:
   apply simp
   done
 
-
 lemma handle_interrupt_integrity:
   "\<lbrace>integrity aag X st and pas_refined aag and invs
-       and (\<lambda>s. pasMaySendIrqs aag \<or> interrupt_states s irq \<noteq> IRQSignal)
-       and (\<lambda>s. ct_active s \<longrightarrow> is_subject aag (cur_thread s))\<rbrace>
-     handle_interrupt irq
-   \<lbrace>\<lambda>rv. integrity aag X st\<rbrace>"
-  apply (simp add: handle_interrupt_def maskInterrupt_def ackInterrupt_def resetTimer_def
+                       and (\<lambda>s. pasMaySendIrqs aag \<or> interrupt_states s irq \<noteq> IRQSignal)
+                       and (\<lambda>s. ct_active s \<longrightarrow> is_subject aag (cur_thread s))\<rbrace>
+   handle_interrupt irq
+   \<lbrace>\<lambda>_. integrity aag X st\<rbrace>"
+  apply (simp add: handle_interrupt_def
              cong: irq_state.case_cong bind_cong)
   apply (rule conjI; rule impI; rule hoare_pre)
-  apply (wp (once) send_signal_respects get_cap_wp dmo_mol_respects dmo_no_mem_respects
-       | wpc
-       | simp add: get_irq_slot_def get_irq_state_def ackInterrupt_def resetTimer_def
-                   handle_reserved_irq_def)+
+     apply (wp (once) send_signal_respects get_cap_wp dmo_mol_respects dmo_no_mem_respects
+                      ackInterrupt_device_state_inv resetTimer_device_state_inv
+            | wpc
+            | simp add: get_irq_slot_def get_irq_state_def)+
   apply clarsimp
   apply (rule conjI, fastforce)+ \<comment> \<open>valid_objs etc.\<close>
   apply (clarsimp simp: cte_wp_at_caps_of_state)
@@ -537,243 +621,132 @@ lemma handle_interrupt_integrity:
   apply assumption+
   done
 
-lemma handle_vm_fault_integrity:
-  "\<lbrace>integrity aag X st and K (is_subject aag thread)\<rbrace>
-    handle_vm_fault thread vmfault_type
-   \<lbrace>\<lambda>rv. integrity aag X st\<rbrace>"
-  apply (cases vmfault_type, simp_all)
-  apply (rule hoare_pre)
-  apply (wp as_user_integrity_autarch dmo_wp | simp add: getDFSR_def getFAR_def getIFSR_def)+
-  done
-
-lemma handle_vm_pas_refined[wp]:
-  "\<lbrace>pas_refined aag\<rbrace>
-    handle_vm_fault thread vmfault_type
-   \<lbrace>\<lambda>rv. pas_refined aag\<rbrace>"
-  apply (cases vmfault_type, simp_all)
-  apply (wp | simp)+
-  done
-
-crunch pas_refined[wp]: handle_hypervisor_fault "pas_refined aag"
-crunch cur_thread[wp]: handle_hypervisor_fault "\<lambda>s. P (cur_thread s)"
-crunch integrity[wp]: handle_hypervisor_fault "integrity aag X st"
-
-lemma handle_vm_cur_thread [wp]:
-  "\<lbrace>\<lambda>s. P (cur_thread s)\<rbrace>
-    handle_vm_fault thread vmfault_type
-   \<lbrace>\<lambda>rv s. P (cur_thread s)\<rbrace>"
-  apply (cases vmfault_type, simp_all)
-  apply (wp | simp)+
-  done
-
-lemma handle_vm_state_refs_of [wp]:
-  "\<lbrace>\<lambda>s. P (state_refs_of s)\<rbrace>
-    handle_vm_fault thread vmfault_type
-   \<lbrace>\<lambda>rv s. P (state_refs_of s)\<rbrace>"
-  apply (cases vmfault_type, simp_all)
-  apply (wp | simp)+
-  done
-
 lemma handle_yield_pas_refined[wp]:
-  "\<lbrace>pas_refined aag\<rbrace>
-    handle_yield
-   \<lbrace>\<lambda>rv. pas_refined aag\<rbrace>"
+  "handle_yield \<lbrace>pas_refined aag\<rbrace>"
   by (simp add: handle_yield_def | wp)+
-
-
 
 lemma handle_event_pas_refined:
   "\<lbrace>pas_refined aag and guarded_pas_domain aag and domain_sep_inv (pasMaySendIrqs aag) st'
-          and einvs and schact_is_rct
-          and (\<lambda>s. ev \<noteq> Interrupt \<longrightarrow> is_subject aag (cur_thread s))
-          and (\<lambda>s. ev \<noteq> Interrupt \<longrightarrow> ct_active s) \<rbrace>
-    handle_event ev
-   \<lbrace>\<lambda>rv. pas_refined aag\<rbrace>"
+                    and einvs and schact_is_rct
+                    and (\<lambda>s. ev \<noteq> Interrupt \<longrightarrow> is_subject aag (cur_thread s))
+                    and (\<lambda>s. ev \<noteq> Interrupt \<longrightarrow> ct_active s) \<rbrace>
+   handle_event ev
+   \<lbrace>\<lambda>_. pas_refined aag\<rbrace>"
   apply (case_tac ev; simp)
       apply (rename_tac syscall)
       apply (case_tac syscall; simp add: handle_send_def handle_call_def)
             apply ((wp handle_invocation_pas_refined handle_recv_pas_refined
                        handle_fault_pas_refined
-                     | simp | clarsimp)+)
+                    | simp | clarsimp)+)
      apply (fastforce simp: valid_fault_def)
-    apply (wp handle_fault_pas_refined
-            | simp)+
+    apply (wp handle_fault_pas_refined | simp)+
     apply (fastforce simp: valid_fault_def)
    apply (wp handle_interrupt_pas_refined handle_fault_pas_refined
              hoare_vcg_conj_lift hoare_vcg_all_lift
-           | wpc
-           | rule hoare_drop_imps
-           | strengthen invs_vobjs_strgs
-           | simp)+
+          | wpc
+          | rule hoare_drop_imps
+          | strengthen invs_vobjs_strgs
+          | simp)+
   done
 
-lemma valid_fault_Unknown [simp]:
+lemma valid_fault_Unknown[simp]:
   "valid_fault (UnknownSyscallException x)"
   by (simp add: valid_fault_def)
 
-lemma valid_fault_User [simp]:
+lemma valid_fault_User[simp]:
   "valid_fault (UserException word1 word2)"
   by (simp add: valid_fault_def)
-
 
 declare hy_inv[wp del]
 
 lemma handle_yield_integrity[wp]:
   "\<lbrace>integrity aag X st and pas_refined aag and is_subject aag \<circ> cur_thread\<rbrace>
-    handle_yield
-   \<lbrace>\<lambda>rv. integrity aag X st\<rbrace>"
+   handle_yield
+   \<lbrace>\<lambda>_. integrity aag X st\<rbrace>"
   by (simp add: handle_yield_def | wp)+
 
-lemma ct_in_state_machine_state_update[simp]: "ct_in_state s (st\<lparr>machine_state := x\<rparr>) = ct_in_state s st"
-  apply (simp add: ct_in_state_def)
-  done
-
+lemma ct_in_state_machine_state_update[simp]:
+  "ct_in_state s (st\<lparr>machine_state := x\<rparr>) = ct_in_state s st"
+  by (simp add: ct_in_state_def)
 
 lemma handle_event_integrity:
-  "\<lbrace>integrity aag X st and pas_refined aag and guarded_pas_domain aag and domain_sep_inv (pasMaySendIrqs aag) st'
-          and einvs and schact_is_rct
-          and (\<lambda>s. ct_active s \<longrightarrow> is_subject aag (cur_thread s)) and (\<lambda>s. ev \<noteq> Interrupt \<longrightarrow> ct_active s) and ((=) st)\<rbrace>
-    handle_event ev
-   \<lbrace>\<lambda>rv. integrity aag X st\<rbrace>"
-  apply (case_tac "ev \<noteq> Interrupt")
-  apply (case_tac ev; simp)
-      apply (rename_tac syscall)
-      apply (case_tac syscall, simp_all add: handle_send_def handle_call_def)
-      apply (wp handle_recv_integrity handle_invocation_respects
-                handle_reply_respects handle_fault_integrity_autarch
-                handle_interrupt_integrity handle_vm_fault_integrity
-                handle_reply_pas_refined handle_vm_fault_valid_fault
-                handle_reply_valid_sched
-                hoare_vcg_conj_lift hoare_vcg_all_lift alternative_wp select_wp
-           | rule dmo_wp
-           | wpc
-           | simp add: getActiveIRQ_def domain_sep_inv_def
-           | clarsimp
-           | rule conjI hoare_vcg_E_elim
-           | strengthen invs_vobjs_strgs invs_mdb_strgs
-           | fastforce)+
-   done
-
-lemma set_thread_state_restart_to_running_respects:
-  "\<lbrace>integrity aag X st and st_tcb_at ((=) Structures_A.Restart) thread
-          and K (pasMayActivate aag)\<rbrace>
-              do pc \<leftarrow> as_user thread getRestartPC;
-                 as_user thread $ setNextPC pc;
-                 set_thread_state thread Structures_A.thread_state.Running
-              od
+  "\<lbrace>integrity aag X st and pas_refined aag and guarded_pas_domain aag
+                       and domain_sep_inv (pasMaySendIrqs aag) st'
+                       and einvs and schact_is_rct
+                       and (\<lambda>s. ct_active s \<longrightarrow> is_subject aag (cur_thread s))
+                       and (\<lambda>s. ev \<noteq> Interrupt \<longrightarrow> ct_active s) and ((=) st)\<rbrace>
+   handle_event ev
    \<lbrace>\<lambda>_. integrity aag X st\<rbrace>"
-  apply (simp add: set_thread_state_def as_user_def split_def setNextPC_def
-                   getRestartPC_def setRegister_def bind_assoc getRegister_def)
-  apply (wpsimp wp: set_object_wp)
-  apply (clarsimp simp: in_monad fun_upd_def[symmetric] cong: if_cong)
-  apply (cases "is_subject aag thread")
-   apply (cut_tac aag=aag in integrity_update_autarch, simp+)
-  apply (erule integrity_trans)
-  apply (clarsimp simp: integrity_def obj_at_def st_tcb_at_def)
-  apply (clarsimp dest!: get_tcb_SomeD)
-  apply (rule_tac tro_tcb_activate[OF refl refl])
-    apply (simp add: tcb_bound_notification_reset_integrity_def)+
-  done
+  apply (cases ev; simp)
+       apply (unfold handle_send_def handle_call_def)
+  by (wpsimp wp: handle_recv_integrity handle_invocation_respects
+                  handle_reply_respects handle_fault_integrity_autarch
+                  handle_interrupt_integrity handle_vm_fault_integrity
+                  handle_reply_pas_refined handle_vm_fault_valid_fault
+                  handle_reply_valid_sched alternative_wp select_wp
+                  hoare_vcg_conj_lift hoare_vcg_all_lift hoare_drop_imps
+            simp: domain_sep_inv_def
+      | rule dmo_wp hoare_vcg_E_elim
+      | fastforce
+      | (rule hoare_vcg_conj_lift)?, wpsimp wp: getActiveIRQ_inv)+
 
 lemma activate_thread_respects:
   "\<lbrace>integrity aag X st and K (pasMayActivate aag)\<rbrace>
-    activate_thread
-   \<lbrace>\<lambda>rv. integrity aag X st\<rbrace>"
-  apply (simp add: activate_thread_def arch_activate_idle_thread_def)
-  apply (rule hoare_pre)
-  apply (wp set_thread_state_restart_to_running_respects thread_get_wp'
-    | wpc | simp add: arch_activate_idle_thread_def get_thread_state_def)+
+   activate_thread
+   \<lbrace>\<lambda>_. integrity aag X st\<rbrace>"
+  apply (simp add: activate_thread_def get_thread_state_def)
+  apply (wpsimp wp: set_thread_state_restart_to_running_respects thread_get_wp')
   apply (clarsimp simp: st_tcb_at_def obj_at_def)
   done
 
 lemma activate_thread_integrity:
-  "\<lbrace>integrity aag X st and (\<lambda>s. cur_thread s \<noteq> idle_thread s \<longrightarrow> is_subject aag (cur_thread s)) and valid_idle\<rbrace>
-    activate_thread
-   \<lbrace>\<lambda>rv. integrity aag X st\<rbrace>"
-  apply (simp add: activate_thread_def arch_activate_idle_thread_def)
+  "\<lbrace>integrity aag X st and valid_idle and
+    (\<lambda>s. cur_thread s \<noteq> idle_thread s \<longrightarrow> is_subject aag (cur_thread s))\<rbrace>
+   activate_thread
+   \<lbrace>\<lambda>_. integrity aag X st\<rbrace>"
+  apply (simp add: activate_thread_def )
   apply (rule hoare_pre)
-  apply (wp gts_wp set_thread_state_integrity_autarch as_user_integrity_autarch | wpc |  simp add: arch_activate_idle_thread_def)+
-  apply(clarsimp simp: valid_idle_def pred_tcb_at_def obj_at_def)
+  apply (wpsimp wp: gts_wp set_thread_state_integrity_autarch as_user_integrity_autarch)+
+  apply (clarsimp simp: valid_idle_def pred_tcb_at_def obj_at_def)
   done
 
 lemma activate_thread_pas_refined:
-  "\<lbrace> pas_refined aag \<rbrace>
-    activate_thread
-   \<lbrace>\<lambda>rv. pas_refined aag \<rbrace>"
-  unfolding activate_thread_def arch_activate_idle_thread_def
-            get_thread_state_def thread_get_def
-  apply (rule hoare_pre)
-  apply (wp set_thread_state_pas_refined hoare_drop_imps
-             | wpc | simp)+
+  "activate_thread \<lbrace>pas_refined aag\<rbrace>"
+  unfolding activate_thread_def get_thread_state_def thread_get_def
+  apply (wpsimp wp: set_thread_state_pas_refined hoare_drop_imps)
   done
 
-lemma integrity_exclusive_state [iff]:
-  "integrity aag X st (s\<lparr>machine_state := machine_state s \<lparr>exclusive_state := es \<rparr>\<rparr>)
-   = integrity aag X st s"
-  unfolding integrity_def
-  by simp
-
-lemma dmo_clearExMonitor_respects_globals[wp]:
-  "\<lbrace>integrity aag X st\<rbrace>
-    do_machine_op clearExMonitor
-   \<lbrace>\<lambda>_. integrity aag X st\<rbrace>"
-  apply (rule hoare_pre)
-  apply (simp add: clearExMonitor_def | wp dmo_wp)+
-  done
-
-lemma integrity_cur_thread [iff]:
+lemma integrity_cur_thread[iff]:
   "integrity aag X st (s\<lparr>cur_thread := v\<rparr>) = integrity aag X st s"
   unfolding integrity_def by simp
 
 lemma tcb_sched_action_dequeue_integrity_pasMayEditReadyQueues:
   "\<lbrace>integrity aag X st and pas_refined aag and K (pasMayEditReadyQueues aag)\<rbrace>
-    tcb_sched_action tcb_sched_dequeue thread
+   tcb_sched_action tcb_sched_dequeue thread
    \<lbrace>\<lambda>_. integrity aag X st\<rbrace>"
   apply (simp add: tcb_sched_action_def)
   apply wp
-  apply (clarsimp simp: integrity_def integrity_ready_queues_def pas_refined_def tcb_domain_map_wellformed_aux_def etcb_at_def get_etcb_def
-                  split: option.splits)
-  done
-
-lemma as_user_set_register_respects_indirect:
-  "\<lbrace>integrity aag X st and st_tcb_at ((=) Structures_A.Running) thread and
-    K ((\<not> is_subject aag thread \<longrightarrow> st_tcb_at receive_blocked thread st
-           \<and> bound_tcb_at ((=) (Some ntfnptr)) thread st)
-        \<and> (aag_has_auth_to aag Notify ntfnptr)) \<rbrace>
-   as_user thread (setRegister r v)
-   \<lbrace>\<lambda>rv. integrity aag X st\<rbrace>"
-  apply (simp add: as_user_def split_def set_object_def get_object_def)
-  apply wp
-  apply (clarsimp simp: in_monad setRegister_def)
-  apply (cases "is_subject aag thread")
-   apply (erule (1) integrity_update_autarch [unfolded fun_upd_def])
-  apply (clarsimp simp: st_tcb_def2 receive_blocked_def)
-  apply (simp split: thread_state.split_asm)
-  apply (rule send_upd_ctxintegrity [OF disjI2, unfolded fun_upd_def],
-         auto simp: st_tcb_def2 indirect_send_def pred_tcb_def2 dest: sym)
+  apply (clarsimp simp: integrity_def integrity_ready_queues_def pas_refined_def
+                        tcb_domain_map_wellformed_aux_def etcb_at_def get_etcb_def
+                 split: option.splits)
   done
 
 lemma switch_to_thread_respects_pasMayEditReadyQueues:
-  notes tcb_sched_action_dequeue_integrity[wp del]
-  shows
-  "\<lbrace>integrity aag X st and pas_refined aag
-    and K (pasMayEditReadyQueues aag)\<rbrace>
-  switch_to_thread t
-  \<lbrace>\<lambda>rv. integrity aag X st\<rbrace>"
-  unfolding switch_to_thread_def arch_switch_to_thread_def
+  "\<lbrace>integrity aag X st and pas_refined aag and K (pasMayEditReadyQueues aag)\<rbrace>
+   switch_to_thread t
+   \<lbrace>\<lambda>_. integrity aag X st\<rbrace>"
+  unfolding switch_to_thread_def
   apply (simp add: spec_valid_def)
-  apply (wp tcb_sched_action_dequeue_integrity_pasMayEditReadyQueues
-                | simp add: clearExMonitor_def)+
+  apply (wpsimp wp: tcb_sched_action_dequeue_integrity_pasMayEditReadyQueues)
   done
 
 lemma switch_to_thread_respects:
-  "\<lbrace>integrity aag X st and pas_refined aag
-    and K (is_subject aag t) \<rbrace>
-  switch_to_thread t
-  \<lbrace>\<lambda>rv. integrity aag X st\<rbrace>"
-  unfolding switch_to_thread_def arch_switch_to_thread_def
+  "\<lbrace>integrity aag X st and pas_refined aag and K (is_subject aag t) \<rbrace>
+   switch_to_thread t
+   \<lbrace>\<lambda>_. integrity aag X st\<rbrace>"
+  unfolding switch_to_thread_def
   apply (simp add: spec_valid_def)
-  apply (wp | simp add: clearExMonitor_def)+
+  apply wpsimp
   done
 
 text \<open>
@@ -782,26 +755,23 @@ See comment for @{thm tcb_sched_action_dequeue_integrity'}
 \<close>
 lemma switch_to_thread_respects':
   "\<lbrace>integrity aag X st and pas_refined aag
-    and (\<lambda>s. pasSubject aag \<in> pasDomainAbs aag (tcb_domain (the (ekheap s t)))) \<rbrace>
-  switch_to_thread t
-  \<lbrace>\<lambda>rv. integrity aag X st\<rbrace>"
-  unfolding switch_to_thread_def arch_switch_to_thread_def
+                       and (\<lambda>s. pasSubject aag \<in> pasDomainAbs aag (tcb_domain (the (ekheap s t))))\<rbrace>
+   switch_to_thread t
+   \<lbrace>\<lambda>_. integrity aag X st\<rbrace>"
+  unfolding switch_to_thread_def
   apply (simp add: spec_valid_def)
-  apply (wp tcb_sched_action_dequeue_integrity'
-        | simp add: clearExMonitor_def)+
+  apply (wpsimp wp: tcb_sched_action_dequeue_integrity')
   done
 
 lemma switch_to_idle_thread_respects:
-  "\<lbrace>integrity aag X st\<rbrace>
-    switch_to_idle_thread
-  \<lbrace>\<lambda>rv. integrity aag X st\<rbrace>"
-  unfolding switch_to_idle_thread_def arch_switch_to_idle_thread_def
-  by (wp | simp)+
+  "switch_to_idle_thread \<lbrace>integrity aag X st\<rbrace>"
+  unfolding switch_to_idle_thread_def by wpsimp
 
 lemma choose_thread_respects_pasMayEditReadyQueues:
-  "\<lbrace>integrity aag X st and pas_refined aag and einvs and valid_queues and K (pasMayEditReadyQueues aag ) \<rbrace>
-  choose_thread
-  \<lbrace>\<lambda>rv. integrity aag X st\<rbrace>"
+  "\<lbrace>integrity aag X st and pas_refined aag and einvs and valid_queues
+                       and K (pasMayEditReadyQueues aag)\<rbrace>
+   choose_thread
+   \<lbrace>\<lambda>_. integrity aag X st\<rbrace>"
   by (simp add: choose_thread_def guarded_switch_to_def
       | wp switch_to_thread_respects_pasMayEditReadyQueues switch_to_idle_thread_respects gts_wp)+
 
@@ -809,9 +779,9 @@ text \<open>integrity for @{const choose_thread} without @{const pasMayEditReady
 lemma choose_thread_respects:
   "\<lbrace>integrity aag X st and pas_refined aag and pas_cur_domain aag and einvs and valid_queues\<rbrace>
    choose_thread
-   \<lbrace>\<lambda>rv. integrity aag X st\<rbrace>"
+   \<lbrace>\<lambda>_. integrity aag X st\<rbrace>"
   apply (simp add: choose_thread_def guarded_switch_to_def
-        | wp switch_to_thread_respects' switch_to_idle_thread_respects gts_wp)+
+         | wp switch_to_thread_respects' switch_to_idle_thread_respects gts_wp)+
   apply (clarsimp simp: pas_refined_def)
   apply (clarsimp simp: tcb_domain_map_wellformed_aux_def)
   apply (clarsimp simp: valid_queues_def is_etcb_at_def)
@@ -832,29 +802,15 @@ lemma choose_thread_respects:
   done
 
 lemma guarded_switch_to_respects:
-  "\<lbrace> integrity aag X st
-     and pas_refined aag and (\<lambda>s. is_subject aag x)\<rbrace>
+  "\<lbrace>integrity aag X st and pas_refined aag and (\<lambda>s. is_subject aag x)\<rbrace>
    guarded_switch_to x
-   \<lbrace>\<lambda>rv. integrity aag X st\<rbrace>"
-   apply (simp add: guarded_switch_to_def)
-   apply (simp add: choose_thread_def guarded_switch_to_def
-               | wp switch_to_thread_respects switch_to_idle_thread_respects gts_wp)+
-   done
+   \<lbrace>\<lambda>_. integrity aag X st\<rbrace>"
+   by (wpsimp simp: guarded_switch_to_def choose_thread_def
+                wp: switch_to_thread_respects switch_to_idle_thread_respects gts_wp)
 
-lemma next_domain_integrity [wp]:
-  "\<lbrace>integrity aag X st\<rbrace>
-  next_domain
-  \<lbrace>\<lambda>rv. integrity aag X st\<rbrace>"
-  apply (simp add: next_domain_def thread_set_domain_def ethread_set_def set_eobject_def Let_def | wp)+
-  apply (clarsimp simp: get_etcb_def integrity_subjects_def lfp_def)
-  done
-
-lemma next_domain_tcb_domain_map_wellformed [wp]:
-  "\<lbrace>tcb_domain_map_wellformed aag\<rbrace>
-  next_domain
-  \<lbrace>\<lambda>rv. tcb_domain_map_wellformed aag\<rbrace>"
-  by (simp add: next_domain_def thread_set_domain_def ethread_set_def set_eobject_def Let_def | wp)+
-
+lemma next_domain_tcb_domain_map_wellformed[wp]:
+  "next_domain \<lbrace>tcb_domain_map_wellformed aag\<rbrace>"
+  by (wpsimp simp: next_domain_def thread_set_domain_def ethread_set_def set_eobject_def Let_def)
 
 lemma valid_blocked_2_valid_blocked_except[simp]:
   "valid_blocked_2 queues kh sa ct \<Longrightarrow> valid_blocked_except_2 t queues kh sa ct"
@@ -862,7 +818,7 @@ lemma valid_blocked_2_valid_blocked_except[simp]:
 
 (* clagged from Schedule_R *)
 lemma next_domain_valid_sched:
-  "\<lbrace> valid_sched and (\<lambda>s. scheduler_action s  = choose_new_thread)\<rbrace> next_domain \<lbrace> \<lambda>_. valid_sched \<rbrace>"
+  "\<lbrace>valid_sched and (\<lambda>s. scheduler_action s = choose_new_thread)\<rbrace> next_domain \<lbrace>\<lambda>_. valid_sched\<rbrace>"
   apply (simp add: next_domain_def Let_def)
   apply (wp, simp add: valid_sched_def valid_sched_action_2_def ct_not_in_q_2_def)
   apply (simp add:valid_blocked_2_def)
@@ -874,10 +830,10 @@ because t's domain may contain multiple labels. See the comment for
 @{thm tcb_sched_action_dequeue_integrity'}
 \<close>
 lemma valid_sched_action_switch_subject_thread:
-   "\<lbrakk> scheduler_action s = switch_thread t ; valid_sched_action s ;
-      valid_etcbs s ; pas_refined aag s ; pas_cur_domain aag s \<rbrakk>
-    \<Longrightarrow> pasObjectAbs aag t \<in> pasDomainAbs aag (tcb_domain (the (ekheap s t))) \<and>
-        pasSubject aag \<in> pasDomainAbs aag (tcb_domain (the (ekheap s t)))"
+   "\<lbrakk> scheduler_action s = switch_thread t; valid_sched_action s;
+      valid_etcbs s; pas_refined aag s; pas_cur_domain aag s \<rbrakk>
+      \<Longrightarrow> pasObjectAbs aag t \<in> pasDomainAbs aag (tcb_domain (the (ekheap s t))) \<and>
+          pasSubject aag \<in> pasDomainAbs aag (tcb_domain (the (ekheap s t)))"
   apply (clarsimp simp: valid_sched_action_def weak_valid_sched_action_2_def
                         switch_in_cur_domain_2_def in_cur_domain_2_def valid_etcbs_def
                         etcb_at_def st_tcb_at_def obj_at_def is_etcb_at_def)
@@ -887,13 +843,33 @@ lemma valid_sched_action_switch_subject_thread:
   apply force
   done
 
+lemma next_domain_integrity[wp]:
+  "next_domain \<lbrace>integrity aag X st\<rbrace>"
+  apply (wpsimp simp: next_domain_def thread_set_domain_def ethread_set_def set_eobject_def Let_def)
+  apply (clarsimp simp: get_etcb_def integrity_subjects_def lfp_def)
+  done
+
+lemma pas_refined_cur_thread[iff]:
+  "pas_refined aag (s\<lparr>cur_thread := v\<rparr>) = pas_refined aag s"
+  unfolding pas_refined_def
+  by (simp add: state_objs_to_policy_def)
+
+lemma switch_to_thread_pas_refined:
+  "switch_to_thread t \<lbrace>pas_refined aag\<rbrace>"
+  unfolding switch_to_thread_def
+  by (wpsimp wp: do_machine_op_pas_refined)
+
+lemma switch_to_idle_thread_pas_refined:
+  "switch_to_idle_thread \<lbrace>pas_refined aag\<rbrace>"
+  unfolding switch_to_idle_thread_def
+  by (wpsimp wp: do_machine_op_pas_refined)
 
 lemma schedule_choose_new_thread_integrity:
-  "\<lbrace> invs and valid_sched and valid_list and integrity aag X st and pas_refined aag
-     and K (pasMayEditReadyQueues aag)
-     and (\<lambda>s. scheduler_action s = choose_new_thread) \<rbrace>
+  "\<lbrace>invs and valid_sched and valid_list and integrity aag X st and pas_refined aag
+         and K (pasMayEditReadyQueues aag)
+         and (\<lambda>s. scheduler_action s = choose_new_thread)\<rbrace>
    schedule_choose_new_thread
-   \<lbrace>\<lambda>rv. integrity aag X st\<rbrace>"
+   \<lbrace>\<lambda>_. integrity aag X st\<rbrace>"
   unfolding schedule_choose_new_thread_def
   by (wpsimp wp: choose_thread_respects_pasMayEditReadyQueues
                  next_domain_valid_sched next_domain_valid_queues
@@ -902,24 +878,18 @@ lemma schedule_choose_new_thread_integrity:
 lemma schedule_integrity:
   "\<lbrace>einvs and integrity aag X st and pas_refined aag and pas_cur_domain aag
           and (\<lambda>s. domain_time s \<noteq> 0) \<rbrace>
-      schedule
-    \<lbrace>\<lambda>rv. integrity aag X st\<rbrace>"
+   schedule
+   \<lbrace>\<lambda>_. integrity aag X st\<rbrace>"
   apply (simp add: schedule_def)
-  apply (rule hoare_pre)
-  supply ethread_get_wp[wp del]
-  apply (wp|wpc|simp only: schedule_choose_new_thread_def)+
-  apply (wpsimp wp: alternative_wp switch_to_thread_respects' select_wp switch_to_idle_thread_respects
-                 guarded_switch_to_lift choose_thread_respects gts_wp hoare_drop_imps
-                 set_scheduler_action_cnt_valid_sched append_thread_queued enqueue_thread_queued
-                 tcb_sched_action_enqueue_valid_blocked_except
-                 tcb_sched_action_append_integrity'
-            wp_del: ethread_get_wp
-    | wpc
-    | simp add: allActiveTCBs_def schedule_choose_new_thread_def
-    | rule hoare_pre_cont[where a=next_domain])+
+  apply (wpsimp wp: alternative_wp switch_to_thread_respects' select_wp guarded_switch_to_lift
+                    switch_to_idle_thread_respects choose_thread_respects gts_wp hoare_drop_imps
+                    set_scheduler_action_cnt_valid_sched append_thread_queued enqueue_thread_queued
+                    tcb_sched_action_enqueue_valid_blocked_except tcb_sched_action_append_integrity'
+         | simp add: allActiveTCBs_def schedule_choose_new_thread_def
+         | rule hoare_pre_cont[where a=next_domain])+
   apply (auto simp: obj_at_def st_tcb_at_def not_cur_thread_2_def valid_sched_def
-              valid_sched_action_def weak_valid_sched_action_def
-              valid_sched_action_switch_subject_thread schedule_choose_new_thread_def)
+                    valid_sched_action_def weak_valid_sched_action_def
+                    valid_sched_action_switch_subject_thread)
   done
 
 lemma  valid_sched_valid_sched_action:
@@ -927,10 +897,10 @@ lemma  valid_sched_valid_sched_action:
   by (simp add: valid_sched_def)
 
 lemma schedule_integrity_pasMayEditReadyQueues:
-  "\<lbrace>einvs and integrity aag X st and pas_refined aag and guarded_pas_domain aag
-          and K (pasMayEditReadyQueues aag) \<rbrace>
-     schedule
-   \<lbrace>\<lambda>rv. integrity aag X st\<rbrace>"
+  "\<lbrace>einvs and integrity aag X st and pas_refined aag
+          and guarded_pas_domain aag and K (pasMayEditReadyQueues aag)\<rbrace>
+   schedule
+   \<lbrace>\<lambda>_. integrity aag X st\<rbrace>"
   supply ethread_get_wp[wp del]
   supply schedule_choose_new_thread_integrity[wp]
   supply if_split[split del]
@@ -942,46 +912,24 @@ lemma schedule_integrity_pasMayEditReadyQueues:
        (* choose thread *)
        apply wp
       (* switch_to *)
-      apply (wpsimp wp: set_scheduler_action_cnt_valid_sched enqueue_thread_queued append_thread_queued
-                        tcb_sched_action_append_integrity_pasMayEditReadyQueues
+      apply (wpsimp wp: set_scheduler_action_cnt_valid_sched enqueue_thread_queued
+                        append_thread_queued tcb_sched_action_append_integrity_pasMayEditReadyQueues
                         guarded_switch_to_lift switch_to_thread_respects_pasMayEditReadyQueues)+
             (* is_highest_prio *)
             apply (simp add: wrap_is_highest_prio_def)
             apply ((wp (once) hoare_drop_imp)+)[1]
            apply (wpsimp wp: tcb_sched_action_enqueue_valid_blocked_except hoare_vcg_imp_lift' gts_wp)+
   apply (clarsimp simp: if_apply_def2 cong: imp_cong conj_cong)
-
-  apply (safe ; ((solves \<open>clarsimp simp: valid_sched_def not_cur_thread_def valid_sched_action_def
-                                         weak_valid_sched_action_def\<close>
-                )?))
+  apply (safe; ((solves \<open>clarsimp simp: valid_sched_def not_cur_thread_def
+                                        valid_sched_action_def weak_valid_sched_action_def\<close>)?))
    apply (clarsimp simp: obj_at_def pred_tcb_at_def)+
   done
 
-lemma pas_refined_cur_thread [iff]:
-  "pas_refined aag (s\<lparr>cur_thread := v\<rparr>) = pas_refined aag s"
-  unfolding pas_refined_def
-  by (simp add:  state_objs_to_policy_def)
-
-lemma switch_to_thread_pas_refined:
-  "\<lbrace>pas_refined aag\<rbrace>
-    switch_to_thread t
-  \<lbrace>\<lambda>rv. pas_refined aag\<rbrace>"
-  unfolding switch_to_thread_def arch_switch_to_thread_def
-  by (wp do_machine_op_pas_refined | simp)+
-
-lemma switch_to_idle_thread_pas_refined:
-  "\<lbrace>pas_refined aag\<rbrace>
-    switch_to_idle_thread
-  \<lbrace>\<lambda>rv. pas_refined aag\<rbrace>"
-  unfolding switch_to_idle_thread_def arch_switch_to_idle_thread_def
-  by (wp do_machine_op_pas_refined | simp)+
-
-crunch pas_refined[wp]: choose_thread "pas_refined aag" (wp: switch_to_thread_pas_refined switch_to_idle_thread_pas_refined crunch_wps)
+crunch pas_refined[wp]: choose_thread "pas_refined aag"
+  (wp: switch_to_thread_pas_refined switch_to_idle_thread_pas_refined crunch_wps)
 
 lemma schedule_pas_refined:
-  "\<lbrace>pas_refined aag\<rbrace>
-  schedule
-  \<lbrace>\<lambda>rv. pas_refined aag\<rbrace>"
+  "schedule \<lbrace>pas_refined aag\<rbrace>"
   apply (simp add: schedule_def allActiveTCBs_def)
   apply (wp add: alternative_wp guarded_switch_to_lift switch_to_thread_pas_refined select_wp
                   switch_to_idle_thread_pas_refined gts_wp
@@ -994,40 +942,18 @@ lemma schedule_pas_refined:
          | wpc | simp add: schedule_choose_new_thread_def)+
   done
 
-lemma handle_interrupt_arch_state [wp]:
-  "\<lbrace>\<lambda>s :: det_ext state. P (arch_state s)\<rbrace> handle_interrupt irq \<lbrace>\<lambda>_ s. P (arch_state s)\<rbrace>"
-  unfolding handle_interrupt_def
-  apply (rule hoare_if)
-  apply (rule hoare_pre)
-  apply clarsimp
-  apply (wp get_cap_inv dxo_wp_weak send_signal_arch_state
-        | wpc
-        | simp add: get_irq_state_def handle_reserved_irq_def)+
-  done
-
 lemmas sequence_x_mapM_x = mapM_x_def [symmetric]
 
-crunch arch_state [wp]: invoke_untyped "\<lambda>s. P (arch_state s)"
-   (wp: crunch_wps without_preemption_wp syscall_valid do_machine_op_arch hoare_unless_wp
-        preemption_point_inv mapME_x_inv_wp
-     simp: crunch_simps sequence_x_mapM_x
-     ignore: do_machine_op freeMemory clearMemory)
+crunch arch_state [wp]: invoke_untyped "\<lambda>s :: det_ext state. P (arch_state s)"
+  (wp: crunch_wps preemption_point_inv mapME_x_inv_wp simp: crunch_simps sequence_x_mapM_x)
 
-end
-
-crunch_ignore (add:
-  cap_swap_ext cap_move_ext cap_insert_ext empty_slot_ext create_cap_ext tcb_sched_action ethread_set
-  reschedule_required set_thread_state_ext possible_switch_to next_domain
-  set_domain
-  timer_tick set_priority retype_region_ext)
-
-context begin interpretation Arch . (*FIXME: arch_split*)
+crunch_ignore (add: cap_swap_ext cap_move_ext cap_insert_ext create_cap_ext set_thread_state_ext
+                    empty_slot_ext retype_region_ext set_priority ethread_set tcb_sched_action
+                    reschedule_required possible_switch_to next_domain set_domain timer_tick)
 
 lemma zet_zip_contrapos:
   "fst t \<notin> set xs  \<Longrightarrow> t \<notin> set (zip xs ys)"
-  apply (rule ccontr)
-  apply (simp add: set_zip_helper)
-  done
+  by (auto simp: set_zip_helper)
 
 lemma ct_active_update[simp]:
   "ct_active (s\<lparr>cdt := b\<rparr>) = ct_active s"
@@ -1037,63 +963,43 @@ lemma ct_active_update[simp]:
   by (auto simp: st_tcb_at_def ct_in_state_def)
 
 lemma set_cap_ct_active[wp]:
-  "\<lbrace>ct_active\<rbrace>
-    set_cap ptr c
-   \<lbrace>\<lambda>_. ct_active \<rbrace>"
+  "set_cap ptr c \<lbrace>ct_active \<rbrace>"
   apply (rule hoare_pre)
-  apply (wp select_wp sts_st_tcb_at_cases thread_set_no_change_tcb_state
-          | simp add: crunch_simps ct_in_state_def | wps)+
+  apply (wps | wpsimp wp: select_wp sts_st_tcb_at_cases thread_set_no_change_tcb_state
+                    simp: crunch_simps ct_in_state_def)+
   done
 
 lemma do_extended_op_ct_active[wp]:
-  "\<lbrace>ct_active\<rbrace>
-    do_extended_op ch
-   \<lbrace>\<lambda>_. ct_active \<rbrace>"
+  "do_extended_op ch \<lbrace>ct_active \<rbrace>"
   apply (rule hoare_pre)
   apply (wp | simp add: crunch_simps ct_in_state_def do_extended_op_def | wps)+
   apply (auto simp: st_tcb_at_def obj_at_def)
   done
 
-crunch ct_active [wp]: set_original "ct_active"
-  ( wp: crunch_wps
-    simp: crunch_simps ct_in_state_def)
-
-crunch ct_active [wp]: set_cdt "ct_active"
-  ( wp: crunch_wps
-    simp: crunch_simps ct_in_state_def)
+crunches set_original, set_cdt
+  for ct_active [wp]: "ct_active"
+  (wp: crunch_wps simp: crunch_simps ct_in_state_def)
 
 lemma cap_swap_ct_active[wp]:
-  "\<lbrace>ct_active\<rbrace>
-    cap_swap a b c d
-   \<lbrace>\<lambda>_. ct_active \<rbrace>"
+  "cap_swap a b c d \<lbrace>ct_active\<rbrace>"
   by (wp | simp add: cap_swap_def | wps)+
 
 lemma unbind_maybe_notification_ct_active[wp]:
-  "\<lbrace>ct_active\<rbrace>
-    unbind_maybe_notification ptr
-   \<lbrace>\<lambda>_. ct_active \<rbrace>"
-  apply (rule hoare_pre)
-  apply (wp | wps | simp add: unbind_maybe_notification_def ct_in_state_def | wpc)+
-  done
+  "unbind_maybe_notification ptr \<lbrace>ct_active\<rbrace>"
+  by (wps | wpsimp simp: unbind_maybe_notification_def ct_in_state_def)+
 
 lemma unbind_notification_ct_active[wp]:
-  "\<lbrace>ct_active\<rbrace>
-    unbind_notification ptr
-   \<lbrace>\<lambda>_. ct_active \<rbrace>"
-  apply (rule hoare_pre)
-  apply (wp | wps | simp add: unbind_notification_def ct_in_state_def | wpc)+
-  done
+  "unbind_notification ptr \<lbrace>ct_active\<rbrace>"
+  by (wps | wpsimp simp: unbind_notification_def ct_in_state_def)+
 
 lemma sts_Restart_ct_active[wp]:
-  "\<lbrace>ct_active\<rbrace> set_thread_state xa Restart \<lbrace>\<lambda>xb. ct_active\<rbrace>"
+  "set_thread_state xa Restart \<lbrace>ct_active\<rbrace>"
   apply (wp set_object_wp | simp add: set_thread_state_def)+
   apply (clarsimp simp: ct_in_state_def st_tcb_at_def obj_at_def)
   done
 
 lemma cancel_all_ipc_ct_active[wp]:
-  "\<lbrace>ct_active\<rbrace>
-    cancel_all_ipc ptr
-   \<lbrace>\<lambda>_. ct_active \<rbrace>"
+  "cancel_all_ipc ptr \<lbrace>ct_active\<rbrace>"
   apply (wp mapM_x_wp set_simple_ko_ct_active | wps | simp add: cancel_all_ipc_def | wpc)+
        apply force
       apply (wp mapM_x_wp set_simple_ko_ct_active)+
@@ -1102,46 +1008,46 @@ lemma cancel_all_ipc_ct_active[wp]:
   apply simp
   done
 
-crunch ct_active [wp]: cap_swap_for_delete "ct_active"
-  ( wp: crunch_wps filterM_preserved hoare_unless_wp
-    simp: crunch_simps ignore: do_extended_op)
+crunch ct_active[wp]: cap_swap_for_delete "ct_active"
+  (wp: crunch_wps filterM_preserved hoare_unless_wp simp: crunch_simps ignore: do_extended_op)
 
-crunch ct_active [wp]: post_cap_deletion, empty_slot "ct_active"
-  ( wp: crunch_wps filterM_preserved hoare_unless_wp
-    simp: crunch_simps ignore: do_extended_op)
+crunch ct_active[wp]: post_cap_deletion, empty_slot "\<lambda>s :: det_ext state. ct_active s"
+  (simp: crunch_simps empty_slot_ext_def ignore: do_extended_op
+     wp: crunch_wps filterM_preserved hoare_unless_wp)
 
-crunch cur_thread[wp]: cap_swap_for_delete,finalise_cap "\<lambda>s. P (cur_thread s)" (wp: select_wp dxo_wp_weak crunch_wps simp: crunch_simps )
+crunch cur_thread[wp]: cap_swap_for_delete, finalise_cap "\<lambda>s :: det_ext state. P (cur_thread s)"
+  (wp: select_wp dxo_wp_weak crunch_wps simp: crunch_simps)
 
-lemma irq_state_indepenedent_cur_thread[simp]: "irq_state_independent_A (\<lambda>s. P (cur_thread s))"
-  by (simp add: irq_state_independent_def)
-
-lemma rec_del_cur_thread[wp]:"\<lbrace>\<lambda>s. P (cur_thread s)\<rbrace> rec_del a \<lbrace>\<lambda>r s. P (cur_thread s)\<rbrace>"
+lemma rec_del_cur_thread[wp]:
+  "rec_del a \<lbrace>\<lambda>s :: det_ext state. P (cur_thread s)\<rbrace>"
   apply (rule rec_del_preservation)
   apply (wp preemption_point_inv|simp)+
   done
 
-crunch cur_thread[wp]: cap_delete,cap_move "\<lambda>s. P (cur_thread s)" (wp: cap_revoke_preservation2 mapM_wp mapM_x_wp crunch_wps dxo_wp_weak simp: filterM_mapM unless_def ignore: without_preemption filterM)
+crunch cur_thread[wp]: cap_delete, cap_move "\<lambda>s :: det_ext state. P (cur_thread s)"
 
-lemma cap_revoke_cur_thread[wp]: "\<lbrace>\<lambda>s. P (cur_thread s)\<rbrace> cap_revoke a \<lbrace>\<lambda>r s. P (cur_thread s)\<rbrace>"
+lemma cap_revoke_cur_thread[wp]:
+  "cap_revoke a \<lbrace>\<lambda>s :: det_ext state. P (cur_thread s)\<rbrace>"
   apply (rule cap_revoke_preservation2)
   apply (wp preemption_point_inv|simp)+
   done
 
-crunch cur_thread[wp]: cancel_badged_sends "\<lambda>s. P (cur_thread s)" (wp: crunch_wps mapM_wp mapM_x_wp dxo_wp_weak simp: filterM_mapM unless_def ignore: without_preemption filterM)
+crunch cur_thread[wp]: cancel_badged_sends "\<lambda>s. P (cur_thread s)"
+  (wp: mapM_wp dxo_wp_weak simp: filterM_mapM)
 
-lemma invoke_cnode_cur_thread[wp]: "\<lbrace>\<lambda>s. P (cur_thread s)\<rbrace> invoke_cnode a \<lbrace>\<lambda>r s. P (cur_thread s)\<rbrace>"
+lemma invoke_cnode_cur_thread[wp]:
+ "invoke_cnode a \<lbrace>\<lambda>s :: det_ext state. P (cur_thread s)\<rbrace>"
   apply (simp add: invoke_cnode_def)
   apply (rule hoare_pre)
   apply (wp hoare_drop_imps hoare_vcg_all_lift | wpc | simp split del: if_split)+
   done
 
-crunch cur_thread[wp]: handle_event "\<lambda>s. P (cur_thread s)"
+crunch cur_thread[wp]: handle_event "\<lambda>s :: det_ext state. P (cur_thread s)"
   (wp: syscall_valid crunch_wps check_cap_inv dxo_wp_weak
-   simp: crunch_simps filterM_mapM
-   ignore: syscall)
+   simp: crunch_simps ignore: syscall)
 
 crunches ethread_set, timer_tick, possible_switch_to, handle_interrupt
-  for pas_cur_domain[wp]: "pas_cur_domain pas"
+  for pas_cur_domain[wp]: "pas_cur_domain aag"
   (wp: crunch_wps simp: crunch_simps ignore_del: ethread_set timer_tick possible_switch_to)
 
 lemma dxo_idle_thread[wp]:
@@ -1151,36 +1057,33 @@ lemma dxo_idle_thread[wp]:
 crunch idle_thread[wp]: throwError "\<lambda>s. P (idle_thread s)"
 
 lemma preemption_point_idle_thread[wp]:
-  "\<lbrace>\<lambda>s. P (idle_thread s) \<rbrace> preemption_point \<lbrace>\<lambda>_ s. P (idle_thread s)\<rbrace>"
-  apply (clarsimp simp: preemption_point_def)
-  by (wpsimp wp: OR_choiceE_weak_wp simp: irq_state_independent_def)
+  "preemption_point \<lbrace>\<lambda>s. P (idle_thread s)\<rbrace>"
+  by (wpsimp wp: OR_choiceE_weak_wp simp: preemption_point_def)
 
-(* following idle_thread and cur_domain proofs clagged from infoflow/PasUpdates.thy *)
-crunch idle_thread'[wp]: cap_delete "\<lambda>s. P (idle_thread s)"
-
-lemma cap_revoke_idle_thread[wp]:"\<lbrace>\<lambda>s. P (idle_thread s)\<rbrace> cap_revoke a \<lbrace>\<lambda>r s. P (idle_thread s)\<rbrace>"
+lemma cap_revoke_idle_thread[wp]:
+  "cap_revoke a \<lbrace>\<lambda>s :: det_ext state. P (idle_thread s)\<rbrace>"
   by (rule cap_revoke_preservation2; wp)
 
-lemma invoke_cnode_idle_thread[wp]: "\<lbrace>\<lambda>s. P (idle_thread s)\<rbrace> invoke_cnode a \<lbrace>\<lambda>r s. P (idle_thread s)\<rbrace>"
+lemma invoke_cnode_idle_thread[wp]:
+  "invoke_cnode a \<lbrace>\<lambda>s :: det_ext state. P (idle_thread s)\<rbrace>"
   apply (simp add: invoke_cnode_def)
   apply (rule hoare_pre)
-    apply (wp hoare_drop_imps hoare_vcg_all_lift | wpc | simp split del: if_split)+
+   apply (wp hoare_drop_imps hoare_vcg_all_lift | wpc | simp split del: if_split)+
   done
 
-crunch idle_thread[wp]: handle_event "\<lambda>s::det_state. P (idle_thread s)"
-  (wp: syscall_valid crunch_wps
-   simp: crunch_simps check_cap_at_def
-   ignore: check_cap_at syscall)
+crunch idle_thread[wp]: handle_event "\<lambda>s :: det_state. P (idle_thread s)"
+  (wp: syscall_valid crunch_wps simp: check_cap_at_def ignore: check_cap_at syscall)
 
 crunch cur_domain[wp]:
-  transfer_caps_loop, ethread_set, possible_switch_to, thread_set_priority, set_priority,
-  set_domain, invoke_domain, cap_move_ext, timer_tick,
+  transfer_caps_loop, ethread_set, possible_switch_to, thread_set_priority,
+  set_priority, set_domain, invoke_domain, cap_move_ext, timer_tick,
   cap_move, cancel_badged_sends, possible_switch_to
   "\<lambda>s. P (cur_domain s)"
-  (wp: crunch_wps simp: crunch_simps filterM_mapM rule: transfer_caps_loop_pres
+  (wp: crunch_wps simp: filterM_mapM rule: transfer_caps_loop_pres
    ignore_del: ethread_set set_priority set_domain cap_move_ext timer_tick possible_switch_to)
 
-lemma invoke_cnode_cur_domain[wp]: "\<lbrace>\<lambda>s. P (cur_domain s)\<rbrace> invoke_cnode a \<lbrace>\<lambda>r s. P (cur_domain s)\<rbrace>"
+lemma invoke_cnode_cur_domain[wp]:
+ "invoke_cnode a \<lbrace>\<lambda>s. P (cur_domain s)\<rbrace>"
   apply (simp add: invoke_cnode_def)
   apply (rule hoare_pre)
    apply (wp hoare_drop_imps hoare_vcg_all_lift | wpc | simp split del: if_split)+
@@ -1192,45 +1095,61 @@ crunch cur_domain[wp]: handle_event "\<lambda>s. P (cur_domain s)"
    ignore: check_cap_at syscall)
 
 lemma handle_event_guarded_pas_domain[wp]:
-  "\<lbrace>guarded_pas_domain aag\<rbrace> handle_event e \<lbrace>\<lambda>_. guarded_pas_domain aag\<rbrace>"
-  by (wp guarded_pas_domain_lift)
+  "handle_event e \<lbrace>guarded_pas_domain aag\<rbrace>"
+  by (wpsimp wp: guarded_pas_domain_lift)
 
 lemma handle_interrupt_guarded_pas_domain[wp]:
-  "\<lbrace>guarded_pas_domain aag\<rbrace> handle_interrupt blah \<lbrace>\<lambda>_. guarded_pas_domain aag\<rbrace>"
-  by (wp guarded_pas_domain_lift)
+  "handle_interrupt blah \<lbrace>guarded_pas_domain aag\<rbrace>"
+  by (wpsimp wp: guarded_pas_domain_lift)
+
+lemma integrity_irq_state_independent[simp]:
+  "integrity_subjects subjects aag activate X st (s\<lparr>machine_state := irq_state_update f ms\<rparr>) =
+   integrity_subjects subjects aag activate X st (s\<lparr>machine_state := ms\<rparr>)"
+  by (clarsimp simp: integrity_def)
+
+lemma guarded_pas_domain_machine_state_update[simp]:
+  "guarded_pas_domain aag (machine_state_update f s) = guarded_pas_domain aag s"
+  by (simp add: guarded_pas_domain_def)
 
 lemma call_kernel_integrity':
   "st \<turnstile> \<lbrace>einvs and pas_refined aag and is_subject aag \<circ> cur_thread and schact_is_rct and guarded_pas_domain aag
-                    and domain_sep_inv (pasMaySendIrqs aag) st'
-                    and (\<lambda>s. ev \<noteq> Interrupt \<longrightarrow> ct_active s) and (ct_active or ct_idle)
-                    and K (pasMayActivate aag \<and> pasMayEditReadyQueues aag)\<rbrace>
-               call_kernel ev
-             \<lbrace>\<lambda>_. integrity aag X st\<rbrace>"
-  apply (simp add: call_kernel_def getActiveIRQ_def )
+               and domain_sep_inv (pasMaySendIrqs aag) st'
+               and (\<lambda>s. ev \<noteq> Interrupt \<longrightarrow> ct_active s) and (ct_active or ct_idle)
+               and K (pasMayActivate aag \<and> pasMayEditReadyQueues aag)\<rbrace>
+        call_kernel ev
+        \<lbrace>\<lambda>_. integrity aag X st\<rbrace>"
+  apply (simp add: call_kernel_def)
   apply (simp only: spec_valid_def)
-  apply (wp activate_thread_respects schedule_integrity_pasMayEditReadyQueues
-            handle_interrupt_integrity
-            dmo_wp alternative_wp select_wp handle_interrupt_pas_refined
-         | simp )+
+  apply (wpsimp wp: activate_thread_respects schedule_integrity_pasMayEditReadyQueues
+                    handle_interrupt_integrity dmo_wp alternative_wp
+                    select_wp handle_interrupt_pas_refined)
+    apply (clarsimp simp: if_fun_split)
+    apply (rule_tac Q="\<lambda>rv ms. (rv \<noteq> None \<longrightarrow> the rv \<notin> non_kernel_IRQs) \<and>
+                                R True (domain_sep_inv (pasMaySendIrqs aag) st' s) rv ms"
+                and R="\<lambda>rv ms. R (the rv \<in> non_kernel_IRQs \<longrightarrow> scheduler_act_sane s \<and> ct_not_queued s)
+                                 (pasMaySendIrqs aag \<or> interrupt_states s (the rv) \<noteq> IRQSignal) rv ms"
+                for R in hoare_strengthen_post[rotated], fastforce simp: domain_sep_inv_def)
+    apply (wpsimp wp: getActiveIRQ_rv_None hoare_drop_imps getActiveIRQ_inv)
    apply (rule hoare_post_impErr,
-          rule_tac Q = "integrity aag X st and pas_refined aag and einvs and guarded_pas_domain aag and domain_sep_inv (pasMaySendIrqs aag) st'
-                        and is_subject aag \<circ> cur_thread
-                        and (\<lambda>_. pasMayActivate aag \<and> pasMayEditReadyQueues aag)" in valid_validE)
-     apply (wp handle_event_integrity he_invs handle_event_pas_refined
-              handle_event_cur_thread handle_event_cur_domain
-              handle_event_domain_sep_inv handle_event_valid_sched | simp)+
-    apply(fastforce simp: domain_sep_inv_def guarded_pas_domain_def)+
+      rule_tac Q="integrity aag X st and pas_refined aag and einvs and guarded_pas_domain aag
+                                     and domain_sep_inv (pasMaySendIrqs aag) st'
+                                     and is_subject aag \<circ> cur_thread
+                                     and K (pasMayActivate aag \<and> pasMayEditReadyQueues aag)"
+            in valid_validE)
+     apply (wpsimp wp: handle_event_integrity he_invs handle_event_pas_refined
+                       handle_event_cur_thread handle_event_cur_domain
+                       handle_event_domain_sep_inv handle_event_valid_sched)+
+    apply (fastforce simp: domain_sep_inv_def guarded_pas_domain_def)+
   done
 
 lemma call_kernel_integrity:
-  "\<lbrace>pas_refined pas and einvs
-    and (\<lambda>s. ev \<noteq> Interrupt \<longrightarrow> ct_active s) and (ct_active or ct_idle)
-    and domain_sep_inv (pasMaySendIrqs pas) st'
-    and schact_is_rct and guarded_pas_domain pas
-    and is_subject pas o cur_thread and K (pasMayActivate pas \<and> pasMayEditReadyQueues pas) and (\<lambda>s. s = st)\<rbrace>
+  "\<lbrace>pas_refined aag and einvs and (\<lambda>s. ev \<noteq> Interrupt \<longrightarrow> ct_active s) and (ct_active or ct_idle)
+                    and domain_sep_inv (pasMaySendIrqs aag) st' and schact_is_rct
+                    and guarded_pas_domain aag and is_subject aag o cur_thread
+                    and K (pasMayActivate aag \<and> pasMayEditReadyQueues aag) and (\<lambda>s. s = st)\<rbrace>
    call_kernel ev
-   \<lbrace>\<lambda>_. integrity pas X st\<rbrace>"
-  using call_kernel_integrity' [of st pas st' ev X]
+   \<lbrace>\<lambda>_. integrity aag X st\<rbrace>"
+  using call_kernel_integrity' [of st st' ev X]
   apply (simp add: spec_valid_def)
   apply (erule hoare_chain)
    apply clarsimp
@@ -1239,17 +1158,16 @@ lemma call_kernel_integrity:
 
 lemma call_kernel_pas_refined:
   "\<lbrace>einvs and pas_refined aag and is_subject aag \<circ> cur_thread and guarded_pas_domain aag
-    and (\<lambda>s. ev \<noteq> Interrupt \<longrightarrow> ct_active s) and (ct_active or ct_idle)
-    and schact_is_rct and pas_cur_domain aag and domain_sep_inv (pasMaySendIrqs aag) st'\<rbrace>
-  call_kernel ev
-  \<lbrace>\<lambda>_. pas_refined aag\<rbrace>"
-  apply (simp add: call_kernel_def getActiveIRQ_def)
+          and (\<lambda>s. ev \<noteq> Interrupt \<longrightarrow> ct_active s) and (ct_active or ct_idle)
+          and schact_is_rct and pas_cur_domain aag and domain_sep_inv (pasMaySendIrqs aag) st'\<rbrace>
+   call_kernel ev
+   \<lbrace>\<lambda>_. pas_refined aag\<rbrace>"
+  apply (simp add: call_kernel_def )
   apply (wp activate_thread_pas_refined schedule_pas_refined handle_interrupt_pas_refined
             do_machine_op_pas_refined dmo_wp alternative_wp select_wp)
-   apply simp
-   apply (rule hoare_post_impErr [OF valid_validE [where Q = "pas_refined aag and invs"]])
-     apply (wp he_invs handle_event_pas_refined)
-    apply auto
+    apply (wpsimp wp: getActiveIRQ_inv)
+   apply (wp he_invs handle_event_pas_refined)
+  apply auto
   done
 
 end
